theories/iris_rules_control.v
@@ -1,0 +1,1364 @@
+From mathcomp Require Import ssreflect eqtype seq ssrbool.
+From iris.program_logic Require Import language.
+From iris.proofmode Require Import base tactics classes.
+From iris.base_logic Require Export gen_heap ghost_map proph_map.
+From iris.base_logic.lib Require Export fancy_updates.
+From iris.bi Require Export weakestpre.
+Require Export iris iris_locations iris_properties iris_atomicity iris_wp_def stdpp_aux.
+Require Export datatypes host operations properties opsem.
+Require Import Coq.Program.Equality.
+
+Lemma wp_br (s : stuckness) (E : coPset) (Φ : val -> iProp Σ) n vs es i LI lh f0:
+  const_list vs ->
+  length vs = n ->
+  lfilled i lh (vs ++ [::AI_basic (BI_br i)]) LI ->
+  ↪[frame] f0 -∗
+  ▷ (↪[frame] f0 -∗ WP (vs ++ es) @ s; E {{ v, Φ v ∗ ↪[frame] f0 }})
+  -∗ WP [AI_label n es LI] @ s; E {{ v, Φ v ∗ ↪[frame] f0 }}.
+Proof.
+  iIntros (Hvs Hlen Hfill) "Hf0 HΦ".
+  iApply wp_lift_step => //=.
+  iIntros (σ ns κ κs nt) "Hσ".
+  iApply fupd_frame_l.
+  iSplit.
+  - iPureIntro. destruct s => //=.
+    unfold language.reducible, language.prim_step => /=.
+    exists [], (vs ++ es), σ, [].
+    destruct σ as [[[hs ws] locs] inst].
+    unfold iris.prim_step => /=.
+    repeat split => //.
+    constructor. econstructor =>//.
+  - destruct σ as [[[hs ws] locs] inst] => //=.
+    iApply fupd_mask_intro;[solve_ndisj|].
+    iIntros "Hcls !>" (es1 σ2 efs HStep).
+    iMod "Hcls". iModIntro.
+    destruct σ2 as [[[hs' ws'] locs'] inst'] => //=.
+    destruct HStep as [H [-> ->]].
+    only_one_reduction H;
+    try by assert (lfilled 0 (LH_base vs []) [AI_basic (BI_br i)]
+                    (vs ++ [AI_basic (BI_br i)])) ;
+      first (by unfold lfilled, lfill ; rewrite Hvs ; rewrite app_nil_r) ;
+    destruct (lfilled_trans _ _ _ _ _ _ _ H Hfill) as [lh' Hfill'] ;
+    eapply lfilled_implies_starts in Hfill' => //= ;
+    unfold first_instr in Hstart ; simpl in Hstart ;
+    unfold first_instr in Hfill' ; rewrite Hfill' in Hstart ;
+    inversion Hstart.
+Qed.
+
+Lemma wp_block (s : stuckness) (E : coPset) (Φ : val -> iProp Σ) vs es n m t1s t2s  f0 :
+  const_list vs ->
+  length vs = n ->
+  length t1s = n ->
+  length t2s = m ->
+  ↪[frame] f0 -∗
+  ▷ (↪[frame] f0 -∗ WP [::AI_label m [::] (vs ++ to_e_list es)] @ s; E {{ v, Φ v ∗ ↪[frame] f0 }})
+  -∗ WP (vs ++ [::AI_basic (BI_block (Tf t1s t2s) es)]) @ s; E {{ v, Φ v ∗ ↪[frame] f0 }}.
+Proof.
+  iIntros (Hvs Hlen1 Hlen2 Hlen3) "Hf0 HΦ".
+  iApply wp_lift_step => //=.
+  apply to_val_cat_None2. done.
+  iIntros (σ ns κ κs nt) "Hσ".
+  iApply fupd_frame_l.
+  iSplit.
+  - iPureIntro. destruct s => //=.
+    unfold language.reducible, language.prim_step => /=.
+    eexists [], _, σ, [].
+    destruct σ as [[[hs ws] locs] inst].
+    unfold iris.prim_step => /=.
+    repeat split => //.
+    constructor. econstructor =>//.
+  - destruct σ as [[[hs ws] locs] inst] => //=.
+    iApply fupd_mask_intro;[solve_ndisj|].
+    iIntros "Hcls !>" (es1 σ2 efs HStep).
+    iMod "Hcls". iModIntro.
+    destruct σ2 as [[[hs' ws'] locs'] inst'] => //=.
+    destruct HStep as [H [-> ->]].
+    eapply reduce_det in H as [H | [Hstart | [ [a Hstart] |
+                                               (Hstart & Hstart1 & Hstart2 & Hσ) ]]];
+      last (by eapply r_simple, rs_block) ;
+      first (inversion H; subst; clear H ; by iExists f0; iFrame) ;
+      rewrite first_instr_const in Hstart => //=.
+Qed.
+
+Lemma wp_label_value (s : stuckness) (E : coPset) (Φ : val -> iProp Σ) es m ctx v f0 :
+  iris.to_val es = Some (immV v) -> 
+  ↪[frame] f0 -∗
+  Φ (immV v) -∗ WP [::AI_label m ctx es] @ s; E {{ v, Φ v ∗ ↪[frame] f0 }}.
+Proof.
+  iIntros (Hval) "Hf0 HP".
+  iApply wp_lift_atomic_step => //=.
+  iIntros (σ ns κ κs nt) "Hσ !>".
+  iSplit.
+  - iPureIntro.
+    destruct s => //=.
+    unfold language.reducible, language.prim_step => /=.
+    exists [], es, σ, [].
+    destruct σ as [[[hs ws] locs] inst].
+    unfold iris.prim_step => /=.
+    repeat split => //.
+    apply r_simple.  apply rs_label_const.
+    eapply to_val_const_list. apply Hval.
+  - destruct σ as [[[hs ws] locs] inst] => //=.
+    iIntros "!>" (es1 σ2 efs HStep) "!>".
+    destruct σ2 as [[[hs' ws'] locs'] inst'] => //=.
+    destruct HStep as [H [-> ->]].
+    eapply reduce_det in H as [H | [Hstart | [ [a Hstart] | (Hstart & Hstart1 & Hstart2
+                                                             & Hσ)]]] ;
+      (try by apply r_simple ; apply rs_label_const ;
+       eapply to_val_const_list ; apply Hval) .
+    + (* The only possible case. *)
+      inversion H; subst; clear H.
+      rewrite Hval.
+      iExists f0.
+      iFrame.
+      iSplit => //.
+      by iIntros.
+    (* All of the rest are impossible reductions since es is a value. *)
+    all: try by unfold first_instr in Hstart ; simpl in Hstart ;
+      remember (find_first_some (map first_instr_instr es)) as fes ;
+      destruct fes => //= ;
+                     apply to_val_const_list in Hval ;
+                     eapply starts_implies_not_constant in Hval ; first (by exfalso) ;
+                     unfold first_instr ; rewrite <- Heqfes.
+Qed.
+(* This lemma turned out not being used in wp_label_trap ; leaving it here for possible
+   future usage *)
+(*
+Lemma lfilled_trap_to_val k lh LI :
+  lfilled k lh [AI_trap] LI ->
+  (LI = [AI_trap] \/ to_val LI = None).
+Proof.
+  intro Hfill. destruct k ; unfold lfilled, lfill in Hfill.
+  { destruct lh ; last by false_assumption.
+    destruct (const_list l) ; last by false_assumption.
+    apply b2p in Hfill. subst.
+    induction l.
+    { destruct l0. { left ; by rewrite app_nil_r. }
+      right. unfold to_val, iris.to_val => //=. } 
+    right. destruct IHl as [Htrap | HNone].
+    apply app_eq_unit in Htrap as [[ -> Htrap ] | [ _ Habs]].
+    apply app_eq_unit in Htrap as [[ Habs _ ] | [ _ ->  ]] => //=.
+    destruct a => //=. destruct b => //=.
+    apply app_eq_nil in Habs as [? ?] => //=.
+    replace ((a :: l)%SEQ ++ [AI_trap] ++ l0) with ([a] ++ (l ++ [AI_trap] ++ l0)).
+    by apply to_val_cat_None2. done. }
+  fold lfill in Hfill. destruct lh ; first by false_assumption.
+  destruct (const_list l) ; last by false_assumption.
+  destruct (lfill _ _ _ ) ; last by false_assumption.
+  apply b2p in Hfill. right.
+  subst ; induction l ; first unfold to_val, iris.to_val => //=.
+  replace ((a :: l)%SEQ ++ (AI_label n l0 l2 :: l1)%SEQ) with
+    ([a] ++ (l ++ AI_label n l0 l2 :: l1)) ; last done.
+  by apply to_val_cat_None2.
+Qed.
+  *)
+    
+
+Lemma wp_label_trap (s : stuckness) (E : coPset) (Φ : val -> iProp Σ) es m ctx f0 :
+  iris.to_val es = Some trapV -> 
+  ↪[frame] f0 -∗
+  Φ trapV -∗ WP [::AI_label m ctx es] @ s; E {{ v, Φ v ∗ ↪[frame] f0 }}.
+Proof.
+  iIntros (Hval) "Hf0 HP".
+  iApply wp_lift_atomic_step => //=.
+  iIntros (σ ns κ κs nt) "Hσ !>".
+  iSplit.
+  - iPureIntro.
+    destruct s => //=.
+    unfold language.reducible, language.prim_step => /=.
+    exists [], [AI_trap], σ, [].
+    destruct σ as [[[hs ws] locs] inst].
+    unfold iris.prim_step => /=.
+    repeat split => //.
+    apply to_val_trap_is_singleton in Hval as ->.
+    apply r_simple.  apply rs_label_trap.
+  - apply to_val_trap_is_singleton in Hval as ->.
+    destruct σ as [[[hs ws] locs] inst] => //=.
+    iIntros "!>" (es1 σ2 efs HStep) "!>".
+    destruct σ2 as [[[hs' ws'] locs'] inst'] => //=.
+    destruct HStep as [H [-> ->]].
+    (* Here, the conclusion of reduce_det is not strong enough, so we re-do the proof
+       of this subcase by hand, since in this particular case, we can get a 
+       stronger result *)
+    remember [AI_label m ctx [AI_trap]] as es0.
+    remember {| f_locs := locs ; f_inst := inst |} as f.
+    remember {| f_locs := locs' ; f_inst := inst' |} as f'.
+    rewrite <- app_nil_l in Heqes0.
+    induction H ; (try by inversion Heqes0) ;
+      try by apply app_inj_tail in Heqes0 as [_ Habs] ; inversion Habs.
+    { destruct H ; (try by inversion Heqes0) ;
+        try by apply app_inj_tail in Heqes0 as [_ Habs] ; inversion Habs.
+      - inversion Heqes0 ; subst. inversion H.
+      - inversion Heqes0 ; subst. inversion Heqf' ; subst.
+        iExists f0.
+        iFrame. iSplit => //. by iIntros.
+      - inversion Heqes0 ; subst. simple_filled H1 i lh bef aft n l l'.
+        found_intruse (AI_basic (BI_br 0)) H1 Hxl1.
+        apply in_or_app. right. apply in_or_app. left.
+        apply in_or_app. right => //=. by left.
+      - rewrite Heqes0 in H0. filled_trap H0 Hxl1. }
+    rewrite Heqes0 in H0.
+    unfold lfilled, lfill in H0 ; destruct k.
+    { destruct lh ; last by false_assumption.
+      destruct (const_list l) ; last by false_assumption.
+      apply b2p, Logic.eq_sym in H0 ; simpl in H0.
+      apply app_eq_unit in H0 as [[ -> H0 ] | [_ Habs]].
+      apply app_eq_unit in H0 as [[ -> _] | [-> ->]] => //=.
+      apply test_no_reduce0 in H. by exfalso.
+      unfold lfilled, lfill in H1 ; simpl in H1. apply b2p in H1.
+      rewrite app_nil_r in H1 ; subst.
+      apply IHreduce => //=.
+      apply app_eq_nil in Habs as [-> _].
+      by apply test_no_reduce0 in H. }
+    fold lfill in H0. destruct lh ; first by false_assumption.
+    destruct (const_list l) ; last by false_assumption.
+    remember (lfill _ _ _) as fill ; destruct fill ; last by false_assumption.
+    apply b2p, Logic.eq_sym in H0. simpl in H0.
+    apply app_eq_unit in H0 as [[ _ H0 ] | [ _ Habs]].
+    inversion H0 ; subst.
+    unfold lfill in Heqfill ; destruct k.
+    { destruct lh ; last by inversion Heqfill.
+      destruct (const_list l0) ; inversion Heqfill.
+      apply Logic.eq_sym, app_eq_unit in H3 as [[ _ H3 ]|[ _ Habs]].
+      apply app_eq_unit in H3 as [[ -> _ ]|[ -> _]].
+      by apply test_no_reduce0 in H.
+      by apply test_no_reduce_trap in H.
+      apply app_eq_nil in Habs as [-> _] ; by apply test_no_reduce0 in H. }
+    fold lfill in Heqfill.
+    destruct lh ; first by inversion Heqfill.
+    destruct (const_list l0) ; last by inversion Heqfill.
+    destruct (lfill k lh es) ; inversion Heqfill.
+    found_intruse (AI_label n l1 l3) H3 Hxl1.
+    inversion Habs.
+Qed.
+
+Lemma wp_val_return (s : stuckness) (E : coPset) (Φ : val -> iProp Σ) vs vs' es' es'' n f0 :
+  const_list vs ->
+  ↪[frame] f0 -∗
+  (↪[frame] f0 -∗ WP vs' ++ vs ++ es'' @ s; E {{ v, Φ v ∗ ↪[frame] f0 }})
+  -∗ WP vs @ s; E CTX 1; LH_rec vs' n es' (LH_base [] []) es'' {{ v, Φ v ∗ ↪[frame] f0 }}.
+Proof.
+  iIntros (Hconst) "Hf0 HWP".
+  iLöb as "IH".
+  iIntros (LI Hfill%lfilled_Ind_Equivalent).
+  inversion Hfill;subst.
+  inversion H8;subst.
+  assert (vs' ++ [AI_label n es' ([] ++ vs ++ [])] ++ es''
+          = ((vs' ++ [AI_label n es' ([] ++ vs ++ [])]) ++ es''))%SEQ as ->.
+  { erewrite app_assoc. auto. }
+  apply const_list_is_val in Hconst as [v1 Hv1].
+  apply const_list_is_val in H7 as [v2 Hv2].
+  eapply to_val_cat_inv in Hv1 as Hvv;[|apply Hv2].
+  iApply (wp_seq _ _ _ (λ v, (⌜v = immV (v2 ++ v1)⌝ ∗ ↪[frame] f0)%I)).
+  iSplitR; first by iIntros "(%H & ?)".
+  iSplitR "HWP".
+  - iApply wp_val_app; first by apply Hv2.
+    iSplit; first by iIntros "!> (%H & ?)".
+    iApply (wp_label_value with "[$]") => //=; first by erewrite app_nil_r; apply Hv1 .
+  - iIntros (w) "(-> & Hf0)".
+    erewrite iris.of_to_val => //.
+    rewrite app_assoc.
+    by iApply "HWP".
+Qed.
+
+Lemma wp_base (s : stuckness) (E : coPset) (Φ : val -> iProp Σ) vs vs' es'' :
+  const_list vs ->
+  WP vs' ++ vs ++ es'' @ s; E {{ Φ }}
+  ⊢ WP vs @ s; E CTX 0; LH_base vs' es'' {{ Φ }}.
+Proof.
+  iIntros (Hconst) "HWP".
+  iIntros (LI Hfill%lfilled_Ind_Equivalent).
+  inversion Hfill;subst. iFrame.
+Qed.
+
+Fixpoint push_base (lh : lholed) n es' vs_pre es_post :=
+  match lh with
+  | LH_base vs_pre' es_post' => LH_rec vs_pre' n es' (LH_base vs_pre es_post) es_post'
+  | LH_rec vs m es'' lh' es => LH_rec vs m es'' (push_base lh' n es' vs_pre es_post) es
+  end.
+
+Fixpoint frame_base (lh : lholed) l1 l2 :=
+  match lh with
+  | LH_base vs es => LH_base (vs ++ l1) (l2 ++ es)
+  | LH_rec vs m es' lh' es => LH_rec vs m es' (frame_base lh' l1 l2) es
+  end.
+
+Lemma lfilledInd_push i : ∀ lh n es' es LI l1 l2,
+  const_list l1 ->
+  lfilledInd i lh ([::AI_label n es' (l1 ++ es ++ l2)]) LI ->
+  lfilledInd (S i) (push_base lh n es' l1 l2) es LI.
+Proof.
+  induction i.
+  all: intros lh n es' es LI l1 l2 Hconst Hfill.
+  { inversion Hfill;subst.
+    constructor. auto. constructor. auto.
+    (* apply lfilled_Ind_Equivalent. cbn. rewrite eqseqE app_nil_r. done.  *)}
+  { inversion Hfill;subst. simpl. constructor. auto.
+    apply IHi. auto. auto. }
+Qed.
+Lemma lfilledInd_frame i : ∀ lh l1 es l2 LI,
+    const_list l1 ->
+    lfilledInd i lh (l1 ++ es ++ l2) LI ->
+    lfilledInd i (frame_base lh l1 l2) (es) LI.
+Proof.
+  induction i.
+  all: intros lh l1 es l2 LI Hconst Hfill.
+  { inversion Hfill;subst.
+    assert (vs ++ (l1 ++ es ++ l2) ++ es'
+            = (vs ++ l1) ++ es ++ (l2 ++ es'))%SEQ as ->.
+    { repeat erewrite app_assoc. auto. }
+    constructor. apply const_list_concat;auto. }
+  { inversion Hfill;subst. simpl. constructor. auto.
+    apply IHi. auto. auto. }
+Qed.
+      
+(* Structural lemmas for contexts *)
+
+Lemma wp_base_push (s : stuckness) (E : coPset) (Φ : val -> iProp Σ) es l1 l2 i lh :
+  const_list l1 ->
+  WP es @ s; E CTX i; frame_base lh l1 l2 {{ Φ }}
+  ⊢ WP l1 ++ es ++ l2 @ s; E CTX i; lh {{ Φ }}.
+Proof.
+  iIntros (Hconst) "HWP".
+  iIntros (LI Hfill%lfilled_Ind_Equivalent).
+  apply lfilledInd_frame in Hfill.
+  iDestruct ("HWP" with "[]") as "HWP";[|iFrame].
+  iPureIntro. by apply lfilled_Ind_Equivalent. auto.
+Qed.
+Lemma wp_label_push (s : stuckness) (E : coPset) (Φ : val -> iProp Σ) es i lh n es' l1 l2 :
+  const_list l1 ->
+  WP es @ s; E CTX S i; push_base lh n es' l1 l2 {{ Φ }}
+  ⊢ WP [::AI_label n es' (l1 ++ es ++ l2)] @ s; E CTX i; lh {{ Φ }}.
+Proof.
+  iIntros (Hconst) "HWP".
+  iIntros (LI Hfill%lfilled_Ind_Equivalent).
+  apply lfilledInd_push in Hfill.
+  iDestruct ("HWP" with "[]") as "HWP";[|iFrame].
+  iPureIntro. by apply lfilled_Ind_Equivalent. auto.
+Qed.
+Lemma wp_label_push_nil (s : stuckness) (E : coPset) (Φ : val -> iProp Σ) es i lh n es' :
+  WP es @ s; E CTX S i; push_base lh n es' [] [] {{ Φ }}
+  ⊢ WP [::AI_label n es' es] @ s; E CTX i; lh {{ Φ }}.
+Proof.
+  iIntros "HWP".
+  iDestruct (wp_label_push with "HWP") as "HWP". auto.
+  erewrite app_nil_l. erewrite app_nil_r. done.
+Qed.
+
+(* Structural lemmas for contexts within a local scope *)
+
+Lemma wp_base_push_local (s : stuckness) (E : coPset) (Φ : val -> iProp Σ) es l1 l2 i lh n f :
+  const_list l1 ->
+  WP es @ s; E FRAME n; f CTX i; frame_base lh l1 l2 {{ v, Φ v }}
+  ⊢ WP l1 ++ es ++ l2 @ s; E FRAME n; f CTX i; lh {{ v, Φ v }}.
+Proof.
+  iIntros (Hconst) "HWP".
+  iIntros (LI Hfill%lfilled_Ind_Equivalent).
+  apply lfilledInd_frame in Hfill.
+  iDestruct ("HWP" with "[]") as "HWP";[|iFrame].
+  iPureIntro. by apply lfilled_Ind_Equivalent. auto.
+Qed.
+Lemma wp_label_push_local (s : stuckness) (E : coPset) (Φ : val -> iProp Σ) es i lh n es' l1 l2 m f :
+  const_list l1 ->
+  WP es @ s; E FRAME m; f CTX S i; push_base lh n es' l1 l2 {{ v, Φ v }}
+  ⊢ WP [::AI_label n es' (l1 ++ es ++ l2)] @ s; E FRAME m; f CTX i; lh {{ v, Φ v }}.
+Proof.
+  iIntros (Hconst) "HWP".
+  iIntros (LI Hfill%lfilled_Ind_Equivalent).
+  apply lfilledInd_push in Hfill.
+  iDestruct ("HWP" with "[]") as "HWP";[|iFrame].
+  iPureIntro. by apply lfilled_Ind_Equivalent. auto.
+Qed.
+Lemma wp_label_push_nil_local (s : stuckness) (E : coPset) (Φ : val -> iProp Σ) es i lh n es' m f :
+  WP es @ s; E FRAME m; f CTX S i; push_base lh n es' [] [] {{ v, Φ v }}
+  ⊢ WP [::AI_label n es' es] @ s; E FRAME m; f CTX i; lh {{ v, Φ v }}.
+Proof.
+  iIntros "HWP".
+  iDestruct (wp_label_push_local with "HWP") as "HWP". auto.
+  erewrite app_nil_l. erewrite app_nil_r. done.
+Qed.
+
+Lemma lfilled_to_val i  :
+  ∀ lh es LI, is_Some (iris.to_val LI) ->
+  lfilled i lh es LI ->
+  is_Some (iris.to_val es).
+Proof.
+  induction i.
+   { intros lh es LI [x Hsome] Hfill.
+    apply lfilled_Ind_Equivalent in Hfill.
+    inversion Hfill;subst.
+    destruct (to_val es) eqn:Hnone;eauto.
+    exfalso.
+    apply (to_val_cat_None1 _ es') in Hnone.
+    apply (to_val_cat_None2 vs) in Hnone.
+    rewrite Hnone in Hsome. done.
+  }
+  { intros lh es LI Hsome Hfill.
+    apply lfilled_Ind_Equivalent in Hfill.
+    inversion Hfill;simplify_eq.
+    clear -Hsome. exfalso.
+    induction vs =>//=.
+    simpl in Hsome. by inversion Hsome.
+    simpl in Hsome; inversion Hsome.
+    destruct a =>//=.
+    destruct b =>//=.
+    destruct (iris.to_val (vs ++ [AI_label n es' LI0] ++ es'')%SEQ) eqn:Hcontr.
+    apply IHvs;eauto.
+    rewrite Hcontr in H. done.
+    destruct vs;done.
+  }
+Qed.
+
+Lemma wp_block_ctx (s : stuckness) (E : coPset) (Φ : val -> iProp Σ) (i : nat) (lh : lholed) vs t1s t2s es n m f0:
+  const_list vs ->
+  length vs = n ->
+  length t1s = n ->
+  length t2s = m ->
+  ↪[frame] f0 -∗
+  ▷ (↪[frame] f0 -∗ WP [::AI_label m [::] (vs ++ to_e_list es)] @ s; E CTX i; lh {{ Φ }})
+  -∗ WP (vs ++ [::AI_basic (BI_block (Tf t1s t2s) es)]) @ s; E CTX i; lh {{ Φ }}.
+Proof.
+  iIntros (Hconst Hn Hn' Hm) "Hf0 HWP".
+  iIntros (LI Hfill).
+  destruct (iris.to_val LI) eqn:Hcontr.
+  { apply lfilled_to_val in Hfill as [v' Hv];eauto.
+    assert (iris.to_val [AI_basic (BI_block (Tf t1s t2s) es)] = None) as Hnone;auto.
+    apply (to_val_cat_None2 vs) in Hnone.
+    rewrite Hv in Hnone. done. }
+  unfold wp_wasm_ctx.
+  repeat rewrite wp_unfold /wasm_wp_pre/=.
+  rewrite Hcontr.
+  iIntros (σ ns κ κs nt) "Hσ".
+  iApply fupd_frame_l.
+  iSplit.
+  { iPureIntro. destruct s;auto.
+    apply lfilled_swap with (es':=[::AI_label m [::] (vs ++ to_e_list es)]) in Hfill as Hfill'.
+    destruct Hfill' as [LI' Hfill'].
+    eexists [],_,σ,[]. simpl.
+    destruct σ as [[[hs ws] locs] inst].
+    unfold iris.prim_step => /=.
+    repeat split => //.
+    eapply r_label. apply r_simple. eapply rs_block.
+    apply Hconst. apply Hn. apply Hn'. apply Hm. eauto. eauto. }
+  destruct σ as [[[hs ws] locs] inst] => //=.
+  iApply fupd_mask_intro;[solve_ndisj|].
+  iIntros "Hcls" (es1 σ2 efs HStep) "!>!>!>".
+  iMod "Hcls". iModIntro.
+  destruct σ2 as [[[hs' ws'] locs'] inst'] => //=.
+  apply lfilled_swap with (es':=[::AI_label m [::] (vs ++ to_e_list es)]) in Hfill as Hfill'.
+  destruct Hfill' as [LI' Hfill'].
+  destruct HStep as [H [-> ->]].
+  eapply reduce_det in H as [ H | [Hstart | [ [a Hstart] | (Hstart & Hstart1 & Hstart2
+                                                            & Hσ)]]] ;
+    try by assert (lfilled 0 (LH_base vs []) [AI_basic (BI_block (Tf t1s t2s) es)]
+                  (vs ++ [AI_basic (BI_block (Tf t1s t2s) es)])) ;
+    first (unfold lfilled, lfill ; rewrite Hconst ; by rewrite app_nil_r) ;
+    destruct (lfilled_trans _ _ _ _ _ _ _ H Hfill) as [lh' Hfill''] ;
+    eapply lfilled_implies_starts in Hfill'' ; (try done) ;
+    rewrite Hfill'' in Hstart ; inversion Hstart => //=.
+  2: { eapply r_label. apply r_simple. eapply rs_block;eauto. all: eauto. }
+  inversion H; subst; clear H.
+  iExists f0.
+  iFrame. iSplit => //.
+  iIntros "Hf0".
+  iSpecialize ("HWP" with "[$]").
+  by iSpecialize ("HWP" with "[%]").
+Qed.
+
+
+Lemma first_instr_local es e n f :
+  first_instr es = Some e ->
+  first_instr [AI_local n f es] = Some e.
+Proof.
+  intros Hfirst.
+  induction es.
+  { inversion Hfirst. }
+  { rewrite /first_instr /=.
+    rewrite /first_instr /= in Hfirst.
+    destruct (first_instr_instr a) eqn:Ha;auto.
+    rewrite Hfirst //. }
+Qed.
+  
+Lemma wp_block_local_ctx (s : stuckness) (E : coPset) (Φ : val -> iProp Σ) (i : nat) (lh : lholed) vs t1s t2s es n m n1 f1 f0 :
+  const_list vs ->
+  length vs = n ->
+  length t1s = n ->
+  length t2s = m ->
+  ↪[frame] f0 -∗
+  ▷ (↪[frame] f0 -∗ WP [::AI_label m [::] (vs ++ to_e_list es)] @ s; E FRAME n1; f1 CTX i; lh {{ v, Φ v }})
+  -∗ WP (vs ++ [::AI_basic (BI_block (Tf t1s t2s) es)]) @ s; E FRAME n1; f1 CTX i; lh {{ v, Φ v }}.
+Proof.
+  iIntros (Hconst Hn Hn' Hm) "Hf0 HWP".
+  iIntros (LI Hfill).
+  destruct (iris.to_val LI) eqn:Hcontr.
+  { apply lfilled_to_val in Hfill as [v' Hv];eauto.
+    assert (iris.to_val [AI_basic (BI_block (Tf t1s t2s) es)] = None) as Hnone;auto.
+    apply (to_val_cat_None2 vs) in Hnone.
+    rewrite Hv in Hnone. done. }
+  unfold wp_wasm_ctx.
+  repeat rewrite wp_unfold /wasm_wp_pre/=.
+  (* rewrite Hcontr. *)
+  iIntros (σ ns κ κs nt) "Hσ".
+  iApply fupd_frame_l.
+  iSplit.
+  { iPureIntro. destruct s;auto.
+    apply lfilled_swap with (es':=[::AI_label m [::] (vs ++ to_e_list es)]) in Hfill as Hfill'.
+    destruct Hfill' as [LI' Hfill'].
+    eexists [],_,σ,[]. simpl.
+    destruct σ as [[[hs ws] locs] inst].
+    unfold iris.prim_step => /=.
+    repeat split => //. eapply r_local.
+    eapply r_label. apply r_simple. eapply rs_block.
+    apply Hconst. apply Hn. apply Hn'. apply Hm. eauto. eauto. }
+  destruct σ as [[[hs ws] locs] inst] => //=.
+  iApply fupd_mask_intro;[solve_ndisj|].
+  iIntros "Hcls" (es1 σ2 efs HStep) "!>!>!>".
+  iMod "Hcls". iModIntro.
+  destruct σ2 as [[[hs' ws'] locs'] inst'] => //=.
+  apply lfilled_swap with (es':=[::AI_label m [::] (vs ++ to_e_list es)]) in Hfill as Hfill'.
+  destruct Hfill' as [LI' Hfill'].
+  destruct HStep as [H [-> ->]].
+  assert (first_instr [AI_local n1 f1 LI] = Some (AI_basic (BI_block (Tf t1s t2s) es))) as HH.
+  { apply first_instr_local. eapply starts_with_lfilled;[|apply Hfill].
+    apply first_instr_const;auto. }
+  eapply reduce_det in H as [ H | [Hstart | [ [a Hstart] | (Hstart & Hstart1 & Hstart2
+                                                            & Hσ)]]];
+    try congruence;
+    try by assert (lfilled 0 (LH_base vs []) [AI_basic (BI_block (Tf t1s t2s) es)]
+                  (vs ++ [AI_basic (BI_block (Tf t1s t2s) es)])) ;
+    first (unfold lfilled, lfill ; rewrite Hconst ; by rewrite app_nil_r) ;
+    destruct (lfilled_trans _ _ _ _ _ _ _ H Hfill) as [lh' Hfill''] ;
+    eapply lfilled_implies_starts in Hfill'' ; (try done) ;
+    rewrite Hfill'' in Hstart ; inversion Hstart => //=.
+  2: { eapply r_local. eapply r_label. apply r_simple. eapply rs_block;eauto. all: eauto. }
+  inversion H; subst; clear H.
+  all: iExists f0.
+  all: iFrame. iSplit => //.
+  iIntros "Hf0".
+  iSpecialize ("HWP" with "[$]").
+  by iSpecialize ("HWP" with "[%]").
+Qed.
+
+Lemma wp_br_ctx (s : stuckness) (E : coPset) (Φ : val -> iProp Σ) n vs es i lh vs' es' f0:
+  const_list vs ->
+  length vs = n ->
+  ↪[frame] f0 -∗
+  ▷ (↪[frame] f0 -∗ WP (vs' ++ vs ++ es ++ es') @ s; E {{ Φ }})
+  -∗ WP vs ++ [::AI_basic (BI_br i)] @ s; E CTX S i; LH_rec vs' n es lh es' {{ Φ }}.
+Proof.
+  iIntros (Hvs Hlen) "Hf0 HΦ".
+  iIntros (LI Hfill).
+  destruct (iris.to_val LI) eqn:Hcontr.
+  { apply lfilled_to_val in Hfill as [v' Hv];eauto.
+    assert (iris.to_val [AI_basic (BI_br i)] = None) as Hnone;auto.
+    apply (to_val_cat_None2 (vs)) in Hnone.
+    rewrite Hv in Hnone. done. }
+  iApply wp_lift_step => //=.
+  iIntros (σ ns κ κs nt) "Hσ".
+  iApply fupd_frame_l.
+  iSplit.
+  { apply lfilled_Ind_Equivalent in Hfill. inversion Hfill;subst.
+    iPureIntro. destruct s;auto.
+    apply lfilled_Ind_Equivalent in H8 as Hfill'.
+    apply lfilled_swap with (es':=vs ++ es) in Hfill' as Hfill''.
+    destruct Hfill'' as [LI' Hfill''].    
+    eexists [],_,σ,[].
+    destruct σ as [[[hs ws] locs] inst].
+    unfold iris.prim_step => /=.
+    repeat split => //.   
+    eapply r_label with (lh:=(LH_base vs' es')).
+    2: { erewrite cons_middle. apply lfilled_Ind_Equivalent.
+         econstructor;auto. }
+    2: { apply lfilled_Ind_Equivalent. econstructor;auto. }
+    apply r_simple. eapply rs_br.
+    apply Hvs. auto. eauto. }
+  destruct σ as [[[hs ws] locs] inst] => //=.
+  iApply fupd_mask_intro;[solve_ndisj|].
+  iIntros "Hcls !>" (es1 σ2 efs HStep).
+  iMod "Hcls". iModIntro.
+  destruct σ2 as [[[hs' ws'] locs'] inst'] => //=.
+  apply lfilled_Ind_Equivalent in Hfill. inversion Hfill;subst.
+  apply lfilled_Ind_Equivalent in H8 as Hfill'.
+  apply lfilled_swap with (es':=vs ++ es) in Hfill' as Hfill''.
+  destruct Hfill'' as [LI' Hfill''].    
+  destruct HStep as [H [-> ->]]. 
+  eapply reduce_det in H as [H | [ Hstart | [ [a Hstart] | (Hstart & Hstart1 & Hstart2 &
+                                                              Hσ)]]] ;
+    try by apply lfilled_Ind_Equivalent in Hfill ;
+    assert (lfilled 0 (LH_base vs []) [AI_basic (BI_br i)]
+                    (vs ++ [AI_basic (BI_br i)])) ;
+    first (unfold lfilled, lfill ; rewrite Hvs ; by rewrite app_nil_r) ;
+    destruct (lfilled_trans _ _ _ _ _ _ _ H Hfill) as [lh' Hfilln] ;
+    eapply lfilled_implies_starts in Hfilln ; (try done) ;
+    rewrite Hfilln in Hstart ; inversion Hstart => //=. 
+  2: { eapply r_label with (lh:=(LH_base vs' es')).
+       2: { apply lfilled_Ind_Equivalent.
+            econstructor;auto. }
+       2: { apply lfilled_Ind_Equivalent. econstructor;auto. }
+       apply r_simple. eapply rs_br. apply Hvs. all:eauto. }
+  inversion H; subst; clear H.
+  iExists f0.
+  iFrame. iSplit => //.
+  iIntros "Hf0".
+  iSpecialize ("HΦ" with "[$]").
+  by erewrite !app_assoc.
+Qed.
+
+Lemma wp_br_local_ctx (s : stuckness) (E : coPset) (Φ : val -> iProp Σ) n vs es i lh vs' es' f0 n1 f1 :
+  const_list vs ->
+  length vs = n ->
+  ↪[frame] f0 -∗
+  ▷ (↪[frame] f0 -∗ WP (vs' ++ vs ++ es ++ es') @ s; E FRAME n1; f1 {{ v, Φ v }})
+  -∗ WP vs ++ [::AI_basic (BI_br i)] @ s; E FRAME n1; f1 CTX S i; LH_rec vs' n es lh es' {{ v, Φ v }}.
+Proof.
+  iIntros (Hvs Hlen) "Hf0 HΦ".
+  iIntros (LI Hfill).
+  destruct (iris.to_val LI) eqn:Hcontr.
+  { apply lfilled_to_val in Hfill as [v' Hv];eauto.
+    assert (iris.to_val [AI_basic (BI_br i)] = None) as Hnone;auto.
+    apply (to_val_cat_None2 (vs)) in Hnone.
+    rewrite Hv in Hnone. done. }
+  iApply wp_lift_step => //=.
+  iIntros (σ ns κ κs nt) "Hσ".
+  iApply fupd_frame_l.
+  iSplit.
+  { apply lfilled_Ind_Equivalent in Hfill. inversion Hfill;subst.
+    iPureIntro. destruct s;auto.
+    apply lfilled_Ind_Equivalent in H8 as Hfill'.
+    apply lfilled_swap with (es':=vs ++ es) in Hfill' as Hfill''.
+    destruct Hfill'' as [LI' Hfill''].    
+    eexists [],_,σ,[].
+    destruct σ as [[[hs ws] locs] inst].
+    unfold iris.prim_step => /=.
+    repeat split => //. eapply r_local.
+    eapply r_label with (lh:=(LH_base vs' es')).
+    2: { erewrite cons_middle. apply lfilled_Ind_Equivalent.
+         econstructor;auto. }
+    2: { apply lfilled_Ind_Equivalent. econstructor;auto. }
+    apply r_simple. eapply rs_br.
+    apply Hvs. auto. eauto. }
+  destruct σ as [[[hs ws] locs] inst] => //=.
+  iApply fupd_mask_intro;[solve_ndisj|].
+  iIntros "Hcls !>" (es1 σ2 efs HStep).
+  iMod "Hcls". iModIntro.
+  destruct σ2 as [[[hs' ws'] locs'] inst'] => //=.
+  apply lfilled_Ind_Equivalent in Hfill. inversion Hfill;subst.
+  apply lfilled_Ind_Equivalent in H8 as Hfill'.
+  apply lfilled_swap with (es':=vs ++ es) in Hfill' as Hfill''.
+  destruct Hfill'' as [LI' Hfill''].    
+  destruct HStep as [H [-> ->]].
+  assert (first_instr [AI_local n1 f1 (vs' ++ [AI_label (length vs) es LI0] ++ es')] 
+     = Some (AI_basic (BI_br i))) as HH.
+  { apply lfilled_Ind_Equivalent in Hfill.
+    apply first_instr_local. eapply starts_with_lfilled;[|apply Hfill].
+    apply first_instr_const;auto. }
+  eapply reduce_det in H as [H | [ Hstart | [ [a Hstart] | (Hstart & Hstart1 & Hstart2 &
+                                                              Hσ)]]] ;
+    try congruence;
+    try by apply lfilled_Ind_Equivalent in Hfill ;
+    assert (lfilled 0 (LH_base vs []) [AI_basic (BI_br i)]
+                    (vs ++ [AI_basic (BI_br i)])) ;
+    first (unfold lfilled, lfill ; rewrite Hvs ; by rewrite app_nil_r) ;
+    destruct (lfilled_trans _ _ _ _ _ _ _ H Hfill) as [lh' Hfilln] ;
+    eapply lfilled_implies_starts in Hfilln ; (try done) ;
+    rewrite Hfilln in Hstart ; inversion Hstart => //=. 
+  2: { eapply r_local.
+       eapply r_label with (lh:=(LH_base vs' es')).
+       2: { apply lfilled_Ind_Equivalent.
+            econstructor;auto. }
+       2: { apply lfilled_Ind_Equivalent. econstructor;auto. }
+       apply r_simple. eapply rs_br. apply Hvs. all:eauto. }
+  inversion H; subst; clear H.
+  iExists f0.
+  iFrame. iSplit => //.
+  iIntros "Hf0".
+  iSpecialize ("HΦ" with "[$]").
+  by erewrite !app_assoc.
+Qed.
+
+Lemma wp_loop_ctx (s : stuckness) (E : coPset) (Φ : val -> iProp Σ) vs es n m t1s t2s i lh f0:
+  const_list vs ->
+  length vs = n ->
+  length t1s = n ->
+  length t2s = m ->
+  ↪[frame] f0 -∗
+  ▷ (↪[frame] f0 -∗ WP [::AI_label n [::AI_basic (BI_loop (Tf t1s t2s) es)] (vs ++ to_e_list es)] @ s; E CTX i; lh {{ Φ }})
+  -∗ WP vs ++ [::AI_basic (BI_loop (Tf t1s t2s) es)] @ s; E CTX i; lh {{ Φ }}.
+Proof.
+  iIntros (Hvs Hn Hn' Hm) "Hf0 HP".
+  iIntros (LI Hfill).
+  eapply lfilled_swap in Hfill as Hfill'; destruct Hfill' as [LI' Hfill'].
+  iApply wp_lift_step => //=.
+  { destruct (iris.to_val LI) eqn:Hcontr;auto.
+    apply lfilled_to_val in Hfill;eauto.
+    destruct Hfill as [? Hfill].
+    assert (iris.to_val [AI_basic (BI_loop (Tf t1s t2s) es)] = None) as HH;auto.
+    apply (to_val_cat_None2 vs) in HH. rewrite Hfill in HH. done. }
+  iIntros (σ ns κ κs nt) "Hσ".
+  iApply fupd_frame_l.
+  iSplitR.
+  - iPureIntro.
+    destruct s => //=.
+    unfold language.reducible, language.prim_step => /=.
+    eexists [], LI', σ, [].
+    destruct σ as [[[hs ws] locs] inst].
+    unfold iris.prim_step => /=.
+    repeat split => //.
+    eapply r_label. apply r_simple;eauto. eapply rs_loop;eauto.
+    eauto. eauto.
+  - destruct σ as [[[hs ws] locs] inst] => //=.
+    iApply fupd_mask_intro;[solve_ndisj|].
+    iIntros "Hcls !>" (es1 σ2 efs HStep).
+    iMod "Hcls". iModIntro.
+    destruct σ2 as [[[hs' ws'] locs'] inst'] => //=.
+    destruct HStep as [H [-> ->]].
+    eapply reduce_det in H as [ H | [Hstart | [ [a Hstart] | (Hstart & Hstart1 & Hstart2
+                                                            & Hσ)]]] ;
+    try by assert (lfilled 0 (LH_base vs []) [AI_basic (BI_loop (Tf t1s t2s) es)]
+                  (vs ++ [AI_basic (BI_loop (Tf t1s t2s) es)])) ;
+    first (unfold lfilled, lfill ; rewrite Hvs ; by rewrite app_nil_r) ;
+    destruct (lfilled_trans _ _ _ _ _ _ _ H Hfill) as [lh' Hfill''] ;
+    eapply lfilled_implies_starts in Hfill'' ; (try done) ;
+    rewrite Hfill'' in Hstart ; inversion Hstart => //=.
+    2: { eapply r_label. apply r_simple;eauto. eapply rs_loop;eauto.
+         eauto. eauto. }
+    inversion H; subst; clear H.
+  iExists f0.
+  iFrame. iSplit => //.
+  iIntros "Hf0".
+  iSpecialize ("HP" with "[$]").
+  by iSpecialize ("HP" with "[%]").
+Qed.
+
+Lemma wp_loop_local_ctx (s : stuckness) (E : coPset) (Φ : val -> iProp Σ) vs es n m t1s t2s i lh f0 n1 f1 :
+  const_list vs ->
+  length vs = n ->
+  length t1s = n ->
+  length t2s = m ->
+  ↪[frame] f0 -∗
+  ▷ (↪[frame] f0 -∗ WP [::AI_label n [::AI_basic (BI_loop (Tf t1s t2s) es)] (vs ++ to_e_list es)] @ s; E FRAME n1; f1 CTX i; lh {{ v, Φ v }})
+  -∗ WP vs ++ [::AI_basic (BI_loop (Tf t1s t2s) es)] @ s; E FRAME n1; f1 CTX i; lh {{ v, Φ v }}.
+Proof.
+  iIntros (Hvs Hn Hn' Hm) "Hf0 HP".
+  iIntros (LI Hfill).
+  eapply lfilled_swap in Hfill as Hfill'; destruct Hfill' as [LI' Hfill'].
+  iApply wp_lift_step => //=.
+  (* { destruct (iris.to_val LI) eqn:Hcontr;auto. *)
+  (*   apply lfilled_to_val in Hfill;eauto. *)
+  (*   destruct Hfill as [? Hfill]. *)
+  (*   assert (iris.to_val [AI_basic (BI_loop (Tf t1s t2s) es)] = None) as HH;auto. *)
+  (*   apply (to_val_cat_None2 vs) in HH. rewrite Hfill in HH. done. } *)
+  iIntros (σ ns κ κs nt) "Hσ".
+  iApply fupd_frame_l.
+  iSplitR.
+  - iPureIntro.
+    destruct s => //=.
+    unfold language.reducible, language.prim_step => /=.
+    eexists [], _, σ, [].
+    destruct σ as [[[hs ws] locs] inst].
+    unfold iris.prim_step => /=.
+    repeat split => //. eapply r_local.
+    eapply r_label. apply r_simple;eauto. eapply rs_loop;eauto.
+    eauto. eauto.
+  - destruct σ as [[[hs ws] locs] inst] => //=.
+    iApply fupd_mask_intro;[solve_ndisj|].
+    iIntros "Hcls !>" (es1 σ2 efs HStep).
+    iMod "Hcls". iModIntro.
+    destruct σ2 as [[[hs' ws'] locs'] inst'] => //=.
+    destruct HStep as [H [-> ->]].
+    assert (first_instr [AI_local n1 f1 LI] = Some (AI_basic (BI_loop (Tf t1s t2s) es))) as HH.
+    { apply first_instr_local. eapply starts_with_lfilled;[|apply Hfill].
+      apply first_instr_const. auto. }
+    eapply reduce_det in H as [ H | [Hstart | [ [a Hstart] | (Hstart & Hstart1 & Hstart2
+                                                            & Hσ)]]] ;
+      try congruence;
+      try by assert (lfilled 0 (LH_base vs []) [AI_basic (BI_loop (Tf t1s t2s) es)]
+                  (vs ++ [AI_basic (BI_loop (Tf t1s t2s) es)])) ;
+    first (unfold lfilled, lfill ; rewrite Hvs ; by rewrite app_nil_r) ;
+    destruct (lfilled_trans _ _ _ _ _ _ _ H Hfill) as [lh' Hfill''] ;
+    eapply lfilled_implies_starts in Hfill'' ; (try done) ;
+    rewrite Hfill'' in Hstart ; inversion Hstart => //=.
+    2: { eapply r_local. eapply r_label. apply r_simple;eauto. eapply rs_loop;eauto.
+         eauto. eauto. }
+    inversion H; subst; clear H.
+  iExists f0.
+  iFrame. iSplit => //.
+  iIntros "Hf0".
+  iSpecialize ("HP" with "[$]").
+  by iSpecialize ("HP" with "[%]").
+Qed.
+
+Lemma wp_loop (s : stuckness) (E : coPset) (Φ : val -> iProp Σ) vs es n m t1s t2s f0:
+  const_list vs ->
+  length vs = n ->
+  length t1s = n ->
+  length t2s = m ->
+  ↪[frame] f0 -∗
+  ▷ (↪[frame] f0 -∗ WP [::AI_label n [::AI_basic (BI_loop (Tf t1s t2s) es)] (vs ++ to_e_list es)] @ s; E {{ Φ }})
+  -∗ WP vs ++ [::AI_basic (BI_loop (Tf t1s t2s) es)] @ s; E {{ Φ }}.
+Proof.
+  iIntros (Hvs Hn Hn' Hm) "Hf0 HP".
+  iApply wp_wasm_empty_ctx. iApply (wp_loop_ctx with "[$]") => //.
+  iNext.
+  iIntros "?"; iSpecialize ("HP" with "[$]").
+  by iApply wp_wasm_empty_ctx. 
+Qed.
+
+Lemma wp_if_true_ctx (s : stuckness) (E : coPset) (Φ : val -> iProp Σ) n tf e1s e2s i lh f0:
+  n ≠ Wasm_int.int_zero i32m ->
+  ↪[frame] f0 -∗
+  ▷ (↪[frame] f0 -∗ WP [::AI_basic (BI_block tf e1s)] @ s; E CTX i; lh {{ Φ }})
+  -∗ WP [::AI_basic (BI_const (VAL_int32 n)); AI_basic (BI_if tf e1s e2s)] @ s; E CTX i; lh {{ Φ }}.
+Proof.
+  iIntros (Hn) "Hf0 HP".
+  iIntros (LI Hfill).
+  eapply lfilled_swap in Hfill as Hfill'; destruct Hfill' as [LI' Hfill'].
+  iApply wp_lift_step => //=.
+  { destruct (iris.to_val LI) eqn:Hcontr;auto.
+    apply lfilled_to_val in Hfill;eauto.
+    destruct Hfill as [? Hfill]. simpl in Hfill. done. }
+  iIntros (σ ns κ κs nt) "Hσ".
+  iApply fupd_frame_l.
+  iSplitR.
+  - iPureIntro.
+    destruct s => //=.
+    unfold language.reducible, language.prim_step => /=.
+    eexists [], LI', σ, [].
+    destruct σ as [[[hs ws] locs] inst].
+    unfold iris.prim_step => /=.
+    repeat split => //.
+    eapply r_label. apply r_simple;eauto. eapply rs_if_true;eauto.
+    eauto. eauto.
+  - destruct σ as [[[hs ws] locs] inst] => //=.
+    iApply fupd_mask_intro;[solve_ndisj|].
+    iIntros "Hcls !>" (es1 σ2 efs HStep).
+    iMod "Hcls". iModIntro.
+    destruct σ2 as [[[hs' ws'] locs'] inst'] => //=.
+    destruct HStep as [H [-> ->]].
+    only_one_reduction H.
+    + iExists f0.
+      iFrame.
+      iIntros "?"; iSpecialize ("HP" with "[$]").
+      by iApply "HP".
+    all: by assert (lfilled 0 (LH_base [AI_basic (BI_const (VAL_int32 n))] [])
+                    [AI_basic (BI_if tf e1s e2s)]
+                    [AI_basic (BI_const (VAL_int32 n)) ; AI_basic (BI_if tf e1s e2s)]) ;
+      first (by unfold lfilled, lfill => //= ; rewrite app_nil_r) ;
+    destruct (lfilled_trans _ _ _ _ _ _ _ H Hfill) as [lh' Hfilln] ;
+    eapply lfilled_implies_starts in Hfilln => //= ;
+    rewrite Hfilln in Hstart ; inversion Hstart.
+Qed.
+
+Lemma wp_if_true_local_ctx (s : stuckness) (E : coPset) (Φ : val -> iProp Σ) n tf e1s e2s i lh f0 n1 f1 :
+  n ≠ Wasm_int.int_zero i32m ->
+  ↪[frame] f0 -∗
+  ▷ (↪[frame] f0 -∗ WP [::AI_basic (BI_block tf e1s)] @ s; E FRAME n1; f1 CTX i; lh {{ v, Φ v }})
+  -∗ WP [::AI_basic (BI_const (VAL_int32 n)); AI_basic (BI_if tf e1s e2s)] @ s; E FRAME n1; f1 CTX i; lh {{ v, Φ v }}.
+Proof.
+  iIntros (Hn) "Hf0 HP".
+  iIntros (LI Hfill).
+  eapply lfilled_swap in Hfill as Hfill'; destruct Hfill' as [LI' Hfill'].
+  iApply wp_lift_step => //=.
+  iIntros (σ ns κ κs nt) "Hσ".
+  iApply fupd_frame_l.
+  iSplitR.
+  - iPureIntro.
+    destruct s => //=.
+    unfold language.reducible, language.prim_step => /=.
+    eexists [], _, σ, [].
+    destruct σ as [[[hs ws] locs] inst].
+    unfold iris.prim_step => /=.
+    repeat split => //. eapply r_local.
+    eapply r_label. apply r_simple;eauto. eapply rs_if_true;eauto.
+    eauto. eauto.
+  - destruct σ as [[[hs ws] locs] inst] => //=.
+    iApply fupd_mask_intro;[solve_ndisj|].
+    iIntros "Hcls !>" (es1 σ2 efs HStep).
+    iMod "Hcls". iModIntro.
+    destruct σ2 as [[[hs' ws'] locs'] inst'] => //=.
+    destruct HStep as [H [-> ->]].
+    assert (first_instr [AI_local n1 f1 LI] = Some (AI_basic (BI_if tf e1s e2s))) as HH.
+    { apply first_instr_local. eapply starts_with_lfilled;[|apply Hfill]. auto. }
+    eapply reduce_det in H as [ H | [Hstart | [ [a Hstart] | (Hstart & Hstart1 & Hstart2
+                                                              & Hσ)]]] ;
+      try congruence;
+      try by assert (lfilled 0 (LH_base vs []) [AI_basic (BI_loop (Tf t1s t2s) es)]
+                             (vs ++ [AI_basic (BI_loop (Tf t1s t2s) es)])) ;
+      first (unfold lfilled, lfill ; rewrite Hvs ; by rewrite app_nil_r) ;
+      destruct (lfilled_trans _ _ _ _ _ _ _ H Hfill) as [lh' Hfill''] ;
+      eapply lfilled_implies_starts in Hfill'' ; (try done) ;
+      rewrite Hfill'' in Hstart ; inversion Hstart => //=.
+    2: { eapply r_local. eapply r_label. apply r_simple;eauto. eapply rs_if_true;eauto.
+         eauto. eauto. }
+    inversion H; subst; clear H.
+    iExists f0.
+    iFrame. iSplit => //.
+    iIntros "Hf0".
+    iSpecialize ("HP" with "[$]").
+    by iSpecialize ("HP" with "[%]").
+Qed.
+
+Lemma wp_if_true (s : stuckness) (E : coPset) (Φ : val -> iProp Σ) n tf e1s e2s f0:
+  n ≠ Wasm_int.int_zero i32m ->
+  ↪[frame] f0 -∗
+  ▷ (↪[frame] f0 -∗ WP [::AI_basic (BI_block tf e1s)] @ s; E {{ Φ }})
+  -∗ WP [::AI_basic (BI_const (VAL_int32 n)); AI_basic (BI_if tf e1s e2s)] @ s; E {{ Φ }}.
+Proof.
+  iIntros (?) "Hf0 HP".
+  iApply wp_wasm_empty_ctx. iApply (wp_if_true_ctx with "[$]");eauto.
+  iNext. iIntros "?"; iSpecialize ("HP" with "[$]").
+  by iApply wp_wasm_empty_ctx.
+Qed.
+  
+Lemma wp_if_false_ctx (s : stuckness) (E : coPset) (Φ : val -> iProp Σ) n tf e1s e2s i lh f0:
+  n = Wasm_int.int_zero i32m ->
+  ↪[frame] f0 -∗
+  ▷ (↪[frame] f0 -∗ WP [::AI_basic (BI_block tf e2s)] @ s; E CTX i; lh {{ Φ }})
+  -∗ WP [::AI_basic (BI_const (VAL_int32 n)); AI_basic (BI_if tf e1s e2s)] @ s; E CTX i; lh {{ Φ }}.
+Proof.
+  iIntros (Hn) "Hf0 HP".
+  iIntros (LI Hfill).
+  eapply lfilled_swap in Hfill as Hfill'; destruct Hfill' as [LI' Hfill'].
+  iApply wp_lift_step => //=.
+  { destruct (iris.to_val LI) eqn:Hcontr;auto.
+    apply lfilled_to_val in Hfill;eauto.
+    destruct Hfill as [? Hfill]. simpl in Hfill. done. }
+  iIntros (σ ns κ κs nt) "Hσ".
+  iApply fupd_frame_l.
+  iSplitR.
+  - iPureIntro.
+    destruct s => //=.
+    unfold language.reducible, language.prim_step => /=.
+    eexists [], LI', σ, [].
+    destruct σ as [[[hs ws] locs] inst].
+    unfold iris.prim_step => /=.
+    repeat split => //.
+    eapply r_label. apply r_simple;eauto. eapply rs_if_false;eauto.
+    eauto. eauto.
+  - destruct σ as [[[hs ws] locs] inst] => //=.
+    iApply fupd_mask_intro;[solve_ndisj|].
+    iIntros "Hcls !>" (es1 σ2 efs HStep).
+    iMod "Hcls". iModIntro.
+    destruct σ2 as [[[hs' ws'] locs'] inst'] => //=.
+    destruct HStep as [H [-> ->]].
+    eapply reduce_det in H as [H | [ Hstart | [[ a Hstart ] |
+                                               (Hstart & Hstart1 & Hstart2 & Hσ)]]] ;
+    try by assert (lfilled 0 (LH_base [AI_basic (BI_const (VAL_int32 n))] [])
+                    [AI_basic (BI_if tf e1s e2s)]
+                    [AI_basic (BI_const (VAL_int32 n)) ; AI_basic (BI_if tf e1s e2s)]) ;
+      first (by unfold lfilled, lfill => //= ; rewrite app_nil_r) ;
+    destruct (lfilled_trans _ _ _ _ _ _ _ H Hfill) as [lh' Hfilln] ;
+    eapply lfilled_implies_starts in Hfilln => //= ;
+    rewrite Hfilln in Hstart ; inversion Hstart.
+    2: { eapply r_label. apply r_simple;eauto. eapply rs_if_false;eauto.
+         eauto. eauto. }
+    inversion H; subst; clear H.
+    iExists f0.
+    iFrame.
+    iSplit => //.
+    iIntros "?"; iSpecialize ("HP" with "[$]").
+    by iApply "HP".
+Qed.
+
+Lemma wp_if_false_local_ctx (s : stuckness) (E : coPset) (Φ : val -> iProp Σ) n tf e1s e2s i lh f0 n1 f1 :
+  n = Wasm_int.int_zero i32m ->
+  ↪[frame] f0 -∗
+  ▷ (↪[frame] f0 -∗ WP [::AI_basic (BI_block tf e2s)] @ s; E FRAME n1; f1 CTX i; lh {{ v, Φ v }})
+  -∗ WP [::AI_basic (BI_const (VAL_int32 n)); AI_basic (BI_if tf e1s e2s)] @ s; E FRAME n1; f1 CTX i; lh {{ v, Φ v }}.
+Proof.
+  iIntros (Hn) "Hf0 HP".
+  iIntros (LI Hfill).
+  eapply lfilled_swap in Hfill as Hfill'; destruct Hfill' as [LI' Hfill'].
+  iApply wp_lift_step => //=.
+  iIntros (σ ns κ κs nt) "Hσ".
+  iApply fupd_frame_l.
+  iSplitR.
+  - iPureIntro.
+    destruct s => //=.
+    unfold language.reducible, language.prim_step => /=.
+    eexists [], _, σ, [].
+    destruct σ as [[[hs ws] locs] inst].
+    unfold iris.prim_step => /=.
+    repeat split => //. eapply r_local.
+    eapply r_label. apply r_simple;eauto. eapply rs_if_false;eauto.
+    eauto. eauto.
+  - destruct σ as [[[hs ws] locs] inst] => //=.
+    iApply fupd_mask_intro;[solve_ndisj|].
+    iIntros "Hcls !>" (es1 σ2 efs HStep).
+    iMod "Hcls". iModIntro.
+    destruct σ2 as [[[hs' ws'] locs'] inst'] => //=.
+    destruct HStep as [H [-> ->]].
+    assert (first_instr [AI_local n1 f1 LI] = Some (AI_basic (BI_if tf e1s e2s))) as HH.
+    { apply first_instr_local. eapply starts_with_lfilled;[|apply Hfill];auto. }
+    eapply reduce_det in H as [H | [ Hstart | [[ a Hstart ] |
+                                               (Hstart & Hstart1 & Hstart2 & Hσ)]]] ;
+      try congruence;
+      try by assert (lfilled 0 (LH_base [AI_basic (BI_const (VAL_int32 n))] [])
+                    [AI_basic (BI_if tf e1s e2s)]
+                    [AI_basic (BI_const (VAL_int32 n)) ; AI_basic (BI_if tf e1s e2s)]) ;
+      first (by unfold lfilled, lfill => //= ; rewrite app_nil_r) ;
+    destruct (lfilled_trans _ _ _ _ _ _ _ H Hfill) as [lh' Hfilln] ;
+    eapply lfilled_implies_starts in Hfilln => //= ;
+    rewrite Hfilln in Hstart ; inversion Hstart.
+    2: { eapply r_local. eapply r_label. apply r_simple;eauto. eapply rs_if_false;eauto.
+         eauto. eauto. }
+    inversion H; subst; clear H.
+    iExists f0.
+    iFrame.
+    iSplit => //.
+    iIntros "?"; iSpecialize ("HP" with "[$]").
+    by iApply "HP".
+Qed.
+
+Lemma wp_if_false (s : stuckness) (E : coPset) (Φ : val -> iProp Σ) n tf e1s e2s f0:
+  n = Wasm_int.int_zero i32m ->
+  ↪[frame] f0 -∗
+  ▷ (↪[frame] f0 -∗ WP [::AI_basic (BI_block tf e2s)] @ s; E {{ Φ }})
+  -∗ WP [::AI_basic (BI_const (VAL_int32 n)); AI_basic (BI_if tf e1s e2s)] @ s; E {{ Φ }}.
+Proof.
+  iIntros (?) "Hf0 HP".
+  iApply wp_wasm_empty_ctx. iApply (wp_if_false_ctx with "[$]");eauto.
+  iNext. iIntros "?". iApply wp_wasm_empty_ctx.
+  by iApply "HP".
+Qed.
+
+Lemma wp_br_if_true_ctx (s : stuckness) (E : coPset) (Φ : val -> iProp Σ) n i j lh f0:
+  n ≠ Wasm_int.int_zero i32m ->
+  ↪[frame] f0 -∗
+  ▷ (↪[frame] f0 -∗ WP [::AI_basic (BI_br i)] @ s; E CTX j; lh {{ Φ }})
+  -∗ WP [::AI_basic (BI_const (VAL_int32 n)); AI_basic (BI_br_if i)] @ s; E CTX j; lh {{ Φ }}.
+Proof.
+  iIntros (Hn) "Hf0 HP".
+  iIntros (LI Hfill).
+  eapply lfilled_swap in Hfill as Hfill'; destruct Hfill' as [LI' Hfill'].
+  iApply wp_lift_step => //=.
+  { destruct (iris.to_val LI) eqn:Hcontr;auto.
+    apply lfilled_to_val in Hfill;eauto.
+    destruct Hfill as [? Hfill]. simpl in Hfill. done. }
+  iIntros (σ ns κ κs nt) "Hσ".
+  iApply fupd_frame_l.
+  iSplitR.
+  - iPureIntro.
+    destruct s => //=.
+    unfold language.reducible, language.prim_step => /=.
+    eexists [], LI', σ, [].
+    destruct σ as [[[hs ws] locs] inst].
+    unfold iris.prim_step => /=.
+    repeat split => //.
+    eapply r_label. apply r_simple;eauto. eapply rs_br_if_true;eauto.
+    eauto. eauto.
+  - destruct σ as [[[hs ws] locs] inst] => //=.
+    iApply fupd_mask_intro;[solve_ndisj|].
+    iIntros "Hcls !>" (es1 σ2 efs HStep).
+    iMod "Hcls". iModIntro.
+    destruct σ2 as [[[hs' ws'] locs'] inst'] => //=.
+    destruct HStep as [H [-> ->]].
+    only_one_reduction H ;
+    try by assert (lfilled 0 (LH_base [AI_basic (BI_const (VAL_int32 n))] [])
+                    [AI_basic (BI_br_if i)]
+                    [AI_basic (BI_const (VAL_int32 n)) ; AI_basic (BI_br_if i)]) ;
+      first (by unfold lfilled, lfill => //= ; rewrite app_nil_r) ;
+    destruct (lfilled_trans _ _ _ _ _ _ _ H Hfill) as [lh' Hfilln] ;
+    eapply lfilled_implies_starts in Hfilln => //= ;
+    rewrite Hfilln in Hstart ; inversion Hstart.
+    iExists f0; iFrame.
+    iIntros "?". by iApply ("HP" with "[$]").
+Qed.
+
+Lemma wp_br_if_true_local_ctx (s : stuckness) (E : coPset) (Φ : val -> iProp Σ) n i j lh f0 n1 f1 :
+  n ≠ Wasm_int.int_zero i32m ->
+  ↪[frame] f0 -∗
+  ▷ (↪[frame] f0 -∗ WP [::AI_basic (BI_br i)] @ s; E FRAME n1; f1 CTX j; lh {{ v, Φ v }})
+  -∗ WP [::AI_basic (BI_const (VAL_int32 n)); AI_basic (BI_br_if i)] @ s; E FRAME n1; f1 CTX j; lh {{ v, Φ v }}.
+Proof.
+  iIntros (Hn) "Hf0 HP".
+  iIntros (LI Hfill).
+  eapply lfilled_swap in Hfill as Hfill'; destruct Hfill' as [LI' Hfill'].
+  iApply wp_lift_step => //=.
+  iIntros (σ ns κ κs nt) "Hσ".
+  iApply fupd_frame_l.
+  iSplitR.
+  - iPureIntro.
+    destruct s => //=.
+    unfold language.reducible, language.prim_step => /=.
+    eexists [], _, σ, [].
+    destruct σ as [[[hs ws] locs] inst].
+    unfold iris.prim_step => /=.
+    repeat split => //. eapply r_local.
+    eapply r_label. apply r_simple;eauto. eapply rs_br_if_true;eauto.
+    eauto. eauto.
+  - destruct σ as [[[hs ws] locs] inst] => //=.
+    iApply fupd_mask_intro;[solve_ndisj|].
+    iIntros "Hcls !>" (es1 σ2 efs HStep).
+    iMod "Hcls". iModIntro.
+    destruct σ2 as [[[hs' ws'] locs'] inst'] => //=.
+    destruct HStep as [H [-> ->]].
+    assert (first_instr [AI_local n1 f1 LI] = Some (AI_basic (BI_br_if i))) as HH.
+    { apply first_instr_local. eapply starts_with_lfilled;[|apply Hfill];auto. }
+    eapply reduce_det in H as [H | [ Hstart | [[ a Hstart ] |
+                                               (Hstart & Hstart1 & Hstart2 & Hσ)]]] ;
+      try congruence;
+      try by assert (lfilled 0 (LH_base [AI_basic (BI_const (VAL_int32 n))] [])
+                    [AI_basic (BI_if tf e1s e2s)]
+                    [AI_basic (BI_const (VAL_int32 n)) ; AI_basic (BI_if tf e1s e2s)]) ;
+      first (by unfold lfilled, lfill => //= ; rewrite app_nil_r) ;
+    destruct (lfilled_trans _ _ _ _ _ _ _ H Hfill) as [lh' Hfilln] ;
+    eapply lfilled_implies_starts in Hfilln => //= ;
+    rewrite Hfilln in Hstart ; inversion Hstart.
+    2: { eapply r_local. eapply r_label. apply r_simple;eauto. eapply rs_br_if_true;eauto.
+         eauto. eauto. }
+    inversion H; subst; clear H.
+    iExists f0.
+    iFrame.
+    iSplit => //.
+    iIntros "?"; iSpecialize ("HP" with "[$]").
+    by iApply "HP".
+Qed.
+
+Lemma wp_br_if_true (s : stuckness) (E : coPset) (Φ : val -> iProp Σ) n i f0:
+  n ≠ Wasm_int.int_zero i32m ->
+  ↪[frame] f0 -∗
+  ▷ (↪[frame] f0 -∗ WP [::AI_basic (BI_br i)] @ s; E {{ Φ }})
+  -∗ WP [::AI_basic (BI_const (VAL_int32 n)); AI_basic (BI_br_if i)] @ s; E {{ Φ }}.
+Proof.
+  iIntros (?) "Hf0 HP".
+  iApply wp_wasm_empty_ctx. iApply (wp_br_if_true_ctx with "[$]");eauto.
+  iNext. iIntros "?". iApply wp_wasm_empty_ctx. by iApply ("HP" with "[$]").
+Qed.
+
+(* The following expression reduces to a value reguardless of context, 
+   and thus does not need a context aware version *)
+Lemma wp_br_if_false (s : stuckness) (E : coPset) (Φ : val -> iProp Σ) n i f0:
+  n = Wasm_int.int_zero i32m ->
+  ↪[frame] f0 -∗
+  ▷ Φ (immV [])
+  -∗ WP [::AI_basic (BI_const (VAL_int32 n)); AI_basic (BI_br_if i)] @ s; E {{ Φ }}.
+Proof.
+  iIntros (Hn) "Hf0 HΦ".
+  iApply wp_lift_atomic_step => //=.
+  iIntros (σ ns κ κs nt) "Hσ !>".
+  iSplit.
+  - iPureIntro.
+    destruct s => //=.
+    unfold reducible, language.prim_step => /=.
+    exists [], [], σ, [].
+    destruct σ as [[[hs ws] locs] inst].
+    unfold iris.prim_step => /=.
+    repeat split => //.
+    apply r_simple.
+    subst.
+    by apply rs_br_if_false.
+  - destruct σ as [[[hs ws] locs] inst] => //=.
+    iIntros "!>" (es σ2 efs HStep) "!>".
+    destruct σ2 as [[[hs' ws'] locs'] inst'] => //=.
+    destruct HStep as [H [-> ->]].
+    only_one_reduction H.
+Qed.
+
+
+Lemma wp_br_table_ctx (s : stuckness) (E : coPset) (Φ : val -> iProp Σ) iss c i j k lh f0:
+  ssrnat.leq (S (Wasm_int.nat_of_uint i32m c)) (length iss) ->
+  List.nth_error iss (Wasm_int.nat_of_uint i32m c) = Some j ->
+  ↪[frame] f0 -∗
+  ▷ (↪[frame] f0 -∗ WP [::AI_basic (BI_br j)] @ s; E CTX k; lh {{ Φ }})
+  -∗ WP [::AI_basic (BI_const (VAL_int32 c)); AI_basic (BI_br_table iss i)] @ s; E CTX k; lh {{ Φ }}.
+Proof.
+  iIntros (Hiss Hj) "Hf0 HP".
+  iIntros (LI Hfill).
+  eapply lfilled_swap in Hfill as Hfill'; destruct Hfill' as [LI' Hfill'].
+  iApply wp_lift_step => //=.
+  { destruct (iris.to_val LI) eqn:Hcontr;auto.
+    apply lfilled_to_val in Hfill;eauto.
+    destruct Hfill as [? Hfill]. simpl in Hfill. done. }
+  iIntros (σ ns κ κs nt) "Hσ".
+  iApply fupd_frame_l.
+  iSplitR.
+  - iPureIntro.
+    destruct s => //=.
+    unfold language.reducible, language.prim_step => /=.
+    eexists [], LI', σ, [].
+    destruct σ as [[[hs ws] locs] inst].
+    unfold iris.prim_step => /=.
+    repeat split => //.
+    eapply r_label. apply r_simple;eauto. apply rs_br_table;eauto.
+    eauto. eauto.
+  - destruct σ as [[[hs ws] locs] inst] => //=.
+    iApply fupd_mask_intro;[solve_ndisj|].
+    iIntros "Hcls !>" (es1 σ2 efs HStep).
+    iMod "Hcls". iModIntro.
+    destruct σ2 as [[[hs' ws'] locs'] inst'] => //=.
+    destruct HStep as [H [-> ->]].
+    only_one_reduction H ;
+     try by assert (lfilled 0 (LH_base [AI_basic (BI_const (VAL_int32 c))] [])
+                    [AI_basic (BI_br_table iss i)]
+                    [AI_basic (BI_const (VAL_int32 c)) ; AI_basic (BI_br_table iss i)]) ;
+      first (by unfold lfilled, lfill => //= ; rewrite app_nil_r) ;
+    destruct (lfilled_trans _ _ _ _ _ _ _ H Hfill) as [lh' Hfilln] ;
+    eapply lfilled_implies_starts in Hfilln => //= ;
+    rewrite Hfilln in Hstart ; inversion Hstart.
+    iExists f0; iFrame.
+    iIntros "?"; by iApply ("HP" with "[$]").
+Qed.
+Lemma wp_br_table_local_ctx (s : stuckness) (E : coPset) (Φ : val -> iProp Σ) iss c i j k lh f0 n1 f1 :
+  ssrnat.leq (S (Wasm_int.nat_of_uint i32m c)) (length iss) ->
+  List.nth_error iss (Wasm_int.nat_of_uint i32m c) = Some j ->
+  ↪[frame] f0 -∗
+  ▷ (↪[frame] f0 -∗ WP [::AI_basic (BI_br j)] @ s; E FRAME n1; f1 CTX k; lh {{ v, Φ v }})
+  -∗ WP [::AI_basic (BI_const (VAL_int32 c)); AI_basic (BI_br_table iss i)] @ s; E FRAME n1; f1 CTX k; lh {{ v, Φ v }}.
+Proof.
+  iIntros (Hiss Hj) "Hf0 HP".
+  iIntros (LI Hfill).
+  eapply lfilled_swap in Hfill as Hfill'; destruct Hfill' as [LI' Hfill'].
+  iApply wp_lift_step => //=.
+  iIntros (σ ns κ κs nt) "Hσ".
+  iApply fupd_frame_l.
+  iSplitR.
+  - iPureIntro.
+    destruct s => //=.
+    unfold language.reducible, language.prim_step => /=.
+    eexists [], _, σ, [].
+    destruct σ as [[[hs ws] locs] inst].
+    unfold iris.prim_step => /=.
+    repeat split => //. eapply r_local.
+    eapply r_label. apply r_simple;eauto. apply rs_br_table;eauto.
+    eauto. eauto.
+  - destruct σ as [[[hs ws] locs] inst] => //=.
+    iApply fupd_mask_intro;[solve_ndisj|].
+    iIntros "Hcls !>" (es1 σ2 efs HStep).
+    iMod "Hcls". iModIntro.
+    destruct σ2 as [[[hs' ws'] locs'] inst'] => //=.
+    destruct HStep as [H [-> ->]].
+    assert (first_instr [AI_local n1 f1 LI] = Some (AI_basic (BI_br_table iss i))) as HH.
+    { apply first_instr_local. eapply starts_with_lfilled;[|apply Hfill];auto. }
+    eapply reduce_det in H as [H | [ Hstart | [[ a Hstart ] |
+                                               (Hstart & Hstart1 & Hstart2 & Hσ)]]] ;
+      try congruence;
+      try by assert (lfilled 0 (LH_base [AI_basic (BI_const (VAL_int32 n))] [])
+                    [AI_basic (BI_if tf e1s e2s)]
+                    [AI_basic (BI_const (VAL_int32 n)) ; AI_basic (BI_if tf e1s e2s)]) ;
+      first (by unfold lfilled, lfill => //= ; rewrite app_nil_r) ;
+    destruct (lfilled_trans _ _ _ _ _ _ _ H Hfill) as [lh' Hfilln] ;
+    eapply lfilled_implies_starts in Hfilln => //= ;
+    rewrite Hfilln in Hstart ; inversion Hstart.
+    2: { eapply r_local. eapply r_label. apply r_simple;eauto. eapply rs_br_table;eauto.
+         eauto. eauto. }
+    inversion H; subst; clear H.
+    iExists f0.
+    iFrame.
+    iSplit => //.
+    iIntros "?"; iSpecialize ("HP" with "[$]").
+    by iApply "HP".
+Qed.
+Lemma wp_br_table (s : stuckness) (E : coPset) (Φ : val -> iProp Σ) iss c i j f0:
+  ssrnat.leq (S (Wasm_int.nat_of_uint i32m c)) (length iss) ->
+  List.nth_error iss (Wasm_int.nat_of_uint i32m c) = Some j ->
+  ↪[frame] f0 -∗
+  ▷ (↪[frame] f0 -∗ WP [::AI_basic (BI_br j)] @ s; E {{ Φ }})
+  -∗ WP [::AI_basic (BI_const (VAL_int32 c)); AI_basic (BI_br_table iss i)] @ s; E {{ Φ }}.
+Proof.
+  iIntros (? ?) "Hf0 HP".
+  iApply wp_wasm_empty_ctx. iApply (wp_br_table_ctx with "[$]");eauto.
+  iNext. iIntros "?". iApply wp_wasm_empty_ctx. by iApply ("HP" with "[$]"). 
+Qed.
+
+Lemma wp_br_table_length_ctx (s : stuckness) (E : coPset) (Φ : val -> iProp Σ) iss c i j lh f0:
+  ssrnat.leq (length iss) (Wasm_int.nat_of_uint i32m c) ->
+  ↪[frame] f0 -∗
+  ▷ (↪[frame] f0 -∗ WP [::AI_basic (BI_br i)] @ s; E CTX j; lh {{ Φ }})
+  -∗ WP [::AI_basic (BI_const (VAL_int32 c)); AI_basic (BI_br_table iss i)] @ s; E CTX j; lh {{ Φ }}.
+Proof.
+  iIntros (Hiss) "Hf0 HP".
+  iIntros (LI Hfill).
+  eapply lfilled_swap in Hfill as Hfill'; destruct Hfill' as [LI' Hfill'].
+  iApply wp_lift_step => //=.
+  { destruct (iris.to_val LI) eqn:Hcontr;auto.
+    apply lfilled_to_val in Hfill;eauto.
+    destruct Hfill as [? Hfill]. simpl in Hfill. done. }
+  iIntros (σ ns κ κs nt) "Hσ".
+  iApply fupd_frame_l.
+  iSplitR.
+  - iPureIntro.
+    destruct s => //=.
+    unfold language.reducible, language.prim_step => /=.
+    eexists [], LI', σ, [].
+    destruct σ as [[[hs ws] locs] inst].
+    unfold iris.prim_step => /=.
+    repeat split => //.
+    eapply r_label. apply r_simple;eauto. apply rs_br_table_length;eauto.
+    eauto. eauto.
+  - destruct σ as [[[hs ws] locs] inst] => //=.
+    iApply fupd_mask_intro;[solve_ndisj|].
+    iIntros "Hcls !>" (es1 σ2 efs HStep).
+    iMod "Hcls". iModIntro.
+    destruct σ2 as [[[hs' ws'] locs'] inst'] => //=.
+    destruct HStep as [H [-> ->]].
+    only_one_reduction H ;
+     try by assert (lfilled 0 (LH_base [AI_basic (BI_const (VAL_int32 c))] [])
+                    [AI_basic (BI_br_table iss i)]
+                    [AI_basic (BI_const (VAL_int32 c)) ; AI_basic (BI_br_table iss i)]) ;
+      first (by unfold lfilled, lfill => //= ; rewrite app_nil_r) ;
+    destruct (lfilled_trans _ _ _ _ _ _ _ H Hfill) as [lh' Hfilln] ;
+    eapply lfilled_implies_starts in Hfilln => //= ;
+    rewrite Hfilln in Hstart ; inversion Hstart.
+    iExists f0; iFrame.
+    iIntros "?"; by iApply ("HP" with "[$]").
+Qed.
+Lemma wp_br_table_length_local_ctx (s : stuckness) (E : coPset) (Φ : val -> iProp Σ) iss c i j lh f0 n1 f1 :
+  ssrnat.leq (length iss) (Wasm_int.nat_of_uint i32m c) ->
+  ↪[frame] f0 -∗
+  ▷ (↪[frame] f0 -∗ WP [::AI_basic (BI_br i)] @ s; E FRAME n1; f1 CTX j; lh {{ v, Φ v }})
+  -∗ WP [::AI_basic (BI_const (VAL_int32 c)); AI_basic (BI_br_table iss i)] @ s; E FRAME n1; f1 CTX j; lh {{ v, Φ v }}.
+Proof.
+  iIntros (Hiss) "Hf0 HP".
+  iIntros (LI Hfill).
+  eapply lfilled_swap in Hfill as Hfill'; destruct Hfill' as [LI' Hfill'].
+  iApply wp_lift_step => //=.
+  iIntros (σ ns κ κs nt) "Hσ".
+  iApply fupd_frame_l.
+  iSplitR.
+  - iPureIntro.
+    destruct s => //=.
+    unfold language.reducible, language.prim_step => /=.
+    eexists [], _, σ, [].
+    destruct σ as [[[hs ws] locs] inst].
+    unfold iris.prim_step => /=.
+    repeat split => //. eapply r_local.
+    eapply r_label. apply r_simple;eauto. apply rs_br_table_length;eauto.
+    eauto. eauto.
+  - destruct σ as [[[hs ws] locs] inst] => //=.
+    iApply fupd_mask_intro;[solve_ndisj|].
+    iIntros "Hcls !>" (es1 σ2 efs HStep).
+    iMod "Hcls". iModIntro.
+    destruct σ2 as [[[hs' ws'] locs'] inst'] => //=.
+    destruct HStep as [H [-> ->]].
+    assert (first_instr [AI_local n1 f1 LI] = Some (AI_basic (BI_br_table iss i))) as HH.
+    { apply first_instr_local. eapply starts_with_lfilled;[|apply Hfill];auto. }
+    eapply reduce_det in H as [H | [ Hstart | [[ a Hstart ] |
+                                               (Hstart & Hstart1 & Hstart2 & Hσ)]]] ;
+      try congruence;
+      try by assert (lfilled 0 (LH_base [AI_basic (BI_const (VAL_int32 n))] [])
+                    [AI_basic (BI_if tf e1s e2s)]
+                    [AI_basic (BI_const (VAL_int32 n)) ; AI_basic (BI_if tf e1s e2s)]) ;
+      first (by unfold lfilled, lfill => //= ; rewrite app_nil_r) ;
+    destruct (lfilled_trans _ _ _ _ _ _ _ H Hfill) as [lh' Hfilln] ;
+    eapply lfilled_implies_starts in Hfilln => //= ;
+    rewrite Hfilln in Hstart ; inversion Hstart.
+    2: { eapply r_local. eapply r_label. apply r_simple;eauto. eapply rs_br_table_length;eauto.
+         eauto. eauto. }
+    inversion H; subst; clear H.
+    iExists f0.
+    iFrame.
+    iSplit => //.
+    iIntros "?"; iSpecialize ("HP" with "[$]").
+    by iApply "HP".
+Qed.
+Lemma wp_br_table_length (s : stuckness) (E : coPset) (Φ : val -> iProp Σ) iss c i f0:
+  ssrnat.leq (length iss) (Wasm_int.nat_of_uint i32m c) ->
+  ↪[frame] f0 -∗
+  ▷ (↪[frame] f0 -∗ WP [::AI_basic (BI_br i)] @ s; E {{ Φ }})
+  -∗ WP [::AI_basic (BI_const (VAL_int32 c)); AI_basic (BI_br_table iss i)] @ s; E {{ Φ }}.
+Proof.
+  iIntros (?) "Hf0 HP".
+  iApply wp_wasm_empty_ctx. iApply (wp_br_table_length_ctx with "[$]");eauto.
+  iNext. iIntros "?". iApply wp_wasm_empty_ctx. by iApply ("HP" with "[$]").
+Qed.
