theories/iris_rules_structural.v
@@ -1,0 +1,795 @@
+
+From mathcomp Require Import ssreflect eqtype seq ssrbool.
+From iris.program_logic Require Import language.
+From iris.proofmode Require Import base tactics classes.
+From iris.base_logic Require Export gen_heap ghost_map proph_map.
+From iris.base_logic.lib Require Export fancy_updates.
+From iris.bi Require Export weakestpre.
+Require Export iris iris_locations iris_properties iris_atomicity iris_wp_def stdpp_aux.
+Require Export datatypes host operations properties opsem.
+Require Import Coq.Program.Equality.
+
+
+(* empty lists, frame and context rules *)
+
+Lemma wp_wasm_empty_ctx (s : stuckness) (E : coPset) (Φ : val -> iProp Σ) e :
+  ⊢ WP e @ s ; E {{ Φ }} ∗-∗ WP e @ s ; E CTX_EMPTY {{ Φ }}.
+Proof.
+  iSplit.
+  { iIntros "HWP". iIntros (LI Hfill%lfilled_Ind_Equivalent).
+    inversion Hfill. subst. erewrite app_nil_l; erewrite app_nil_r. done. }
+  { iIntros "HWP".
+    iDestruct ("HWP" $! e with "[]") as "$".
+    iPureIntro. cbn. rewrite app_nil_r eqseqE. apply eq_refl. }
+Qed.
+Lemma wp_wasm_empty_ctx_frame (s : stuckness) (E : coPset) (Φ : val -> iProp Σ) e n f :
+  ⊢ WP e @ s ; E FRAME n; f {{ Φ }} ∗-∗ WP e @ s ; E FRAME n; f CTX_EMPTY {{ v, Φ v }}.
+Proof.
+  iSplit.
+  { iIntros "HWP". iIntros (LI Hfill%lfilled_Ind_Equivalent).
+    inversion Hfill. subst. erewrite app_nil_l; erewrite app_nil_r. done. }
+  { iIntros "HWP".
+    iDestruct ("HWP" $! e with "[]") as "$".
+    iPureIntro. cbn. rewrite app_nil_r eqseqE. apply eq_refl. }
+Qed.
+
+Lemma wp_nil (s : stuckness) (E : coPset) (Φ : iProp Σ) f :
+  ↪[frame] f ∗ Φ ⊢ WP [] @ s ; E CTX_EMPTY {{ fun v => Φ }}%I.
+Proof.
+  iIntros "(Hframe & H)". iApply wp_wasm_empty_ctx.
+  by rewrite wp_unfold /wasm_wp_pre.
+Qed.
+
+Lemma wp_seq_ctx (s : stuckness) (E : coPset) (Φ Ψ : val -> iProp Σ) (es1 es2 : language.expr wasm_lang) (i : nat) (lh : lholed) :
+  (WP es1 @ NotStuck; E {{ w, Ψ w }} ∗
+  ∀ w, Ψ w -∗ WP (iris.of_val w ++ es2) @ s; E CTX i; lh {{ v, Φ v }})%I
+  ⊢ WP (es1 ++ es2) @ s; E CTX i; lh {{ v, Φ v }}.
+Proof.
+  iLöb as "IH" forall (s E es1 es2 Φ Ψ i lh).
+{ iIntros "[Hes1 Hes2]".
+  (* iDestruct (wp_wasm_empty_ctx with "Hes1") as "Hes1". *)
+  iIntros (LI Hfilled).
+  repeat rewrite wp_unfold /wasm_wp_pre /=.
+  (* Base case, when both es1 and es2 are values *)
+  destruct (iris.to_val LI) as [vs|] eqn:Hetov.
+  { destruct vs.
+    { pose proof (filled_is_val_imm _ _ _ _ _ Hetov Hfilled) as
+        [vs [es' [-> [-> [Hconst1 Hconst2]]]]].
+      apply const_list_is_val in Hconst1 as [v1 Hv1].
+      apply const_list_is_val in Hconst2 as [v2 Hv2].
+      edestruct fill_val as [vs12 [Hvs12 Heql]];eauto.
+      assert (Hvs12':=Hvs12).
+      apply to_val_cat in Hvs12' as [-> Hev2].
+      apply iris.of_to_val in Hev2 as <-.
+      iMod "Hes1".
+      iSpecialize ("Hes2" with "Hes1").
+      unfold iris.of_val.
+      rewrite - fmap_app take_drop.
+      rewrite of_val_imm.
+      pose proof (lfilled_swap (iris.of_val (immV vs12)) Hfilled) as [LI' Hfilled'].
+      iSpecialize ("Hes2" $! _ Hfilled').
+      rewrite wp_unfold /wasm_wp_pre /=.
+      assert (iris.to_val LI' = Some (immV l)) as ->;[|iFrame].
+      apply lfilled_Ind_Equivalent in Hfilled'. inversion Hfilled';subst.
+      apply to_val_cat_inv;auto. apply to_val_cat_inv;auto. apply iris.to_of_val.
+    }
+    { apply to_val_trap_is_singleton in Hetov. subst.
+      apply lfilled_Ind_Equivalent in Hfilled.
+      inversion Hfilled;subst.
+      2: { exfalso. do 2 destruct vs =>//=. }
+      apply app_eq_singleton in H as [[HH HH']|[HH HH']];subst.
+      { exfalso. destruct es1,es2,es' =>//=. }
+      apply app_eq_singleton in HH' as [[HH HH']|[HH HH']];subst.
+      { apply app_eq_singleton in HH as [[-> ->]|[-> ->]].
+        simpl.
+        all:iMod "Hes1".
+        all: iSpecialize ("Hes2" with "Hes1").
+        all:rewrite /=.
+        all: iDestruct (wp_wasm_empty_ctx with "Hes2") as "Hes2".
+        all:by rewrite wp_unfold /wasm_wp_pre /=. }
+      { destruct es1,es2 =>//=.
+        iMod "Hes1".
+        iSpecialize ("Hes2" with "Hes1").
+        rewrite /=.
+        iSpecialize ("Hes2" $! [AI_trap] with "[]").
+        { iPureIntro. constructor. }
+        by rewrite wp_unfold /wasm_wp_pre /=.  }
+    }
+  }
+  {
+  (* Ind *)
+  iIntros (σ ns κ κs nt) "Hσ".
+  destruct (iris.to_val es1) as [vs|] eqn:Hes.
+  { apply of_to_val in Hes as <-.
+    iMod "Hes1".
+    iSpecialize ("Hes2" with "Hes1").
+    iSpecialize ("Hes2" $! _ Hfilled).
+    rewrite wp_unfold /wasm_wp_pre /=.
+    rewrite Hetov.
+    iSpecialize ("Hes2" $! σ ns κ κs nt with "[$]").
+    iMod "Hes2" as "[%H1 H2]".
+    iIntros "!>".
+    iSplit.
+    - iPureIntro. by apply H1. 
+    - by iApply "H2".
+  }
+  {
+    iSpecialize ("Hes1" $! σ ns κ κs nt with "[$]").
+    iMod "Hes1" as "[%H1 H2]".
+    iModIntro.
+    iSplit.
+    - iPureIntro.
+      destruct s => //.
+      apply append_reducible with (es2:=es2) in H1;auto.
+      eapply lfilled_reducible. apply Hfilled. auto.
+    - iIntros (e2 σ2 efs HStep').
+      eapply lfilled_prim_step_split_reduce_r in HStep' as Heq;[|apply Hfilled|apply H1].
+      destruct Heq as [e' [HStep'' Hlfilled']].
+      apply prim_step_obs_efs_empty in HStep'' as Hemp. inversion Hemp;subst;clear Hemp.
+      apply prim_step_obs_efs_empty in HStep' as Hemp. inversion Hemp;subst;clear Hemp.
+      iSpecialize ("H2" $! e' σ2 [] HStep'').
+      iMod "H2".
+      repeat iModIntro.
+      repeat iMod "H2".
+      iModIntro.
+      iDestruct "H2" as (f1) "(Hσ & Hf1 & Hes'' & Hefs)".
+      iExists f1.
+      iFrame.
+      iSplit => //.
+      iIntros "?"; iSpecialize ("Hes''" with "[$]").
+      iDestruct ("IH" with "[$Hes'' $Hes2]") as "Hcont".
+      by iApply "Hcont".
+  } } }
+Qed.
+
+(* Contextual rules for Local computation *)
+
+Lemma wp_frame_rewrite (s: stuckness) (E: coPset) (Φ: val -> iProp Σ) es n f:
+  WP es @ s; E FRAME n; f {{ v, Φ v }} ⊣⊢
+  WP [AI_local n f es] @ s; E {{ v, Φ v }}.
+Proof.
+  trivial.
+Qed.
+
+Lemma wp_frame_value (s : stuckness) (E : coPset) (Φ : val -> iProp Σ) es n f f0 vs :
+  iris.to_val es = Some (immV vs) ->
+  length es = n ->
+  ↪[frame] f0 -∗
+  ▷ (↪[frame] f0 -∗ Φ (immV vs)) -∗
+  WP es @ s; E FRAME n; f {{ Φ }}.
+Proof.
+  iIntros (Hv Hlen) "Hframe H".
+  rewrite wp_frame_rewrite.
+  apply to_val_const_list in Hv as Hconst.
+  iApply wp_lift_atomic_step. simpl ; trivial.
+  iIntros (σ ns κ κs nt) "Hσ !>".
+  iSplit.
+  - iPureIntro.
+    destruct s => //=.
+    unfold language.reducible, language.prim_step => /=.
+    exists [], es, σ, [].
+    destruct σ as [[[ hs ws] locs] inst].
+    unfold iris.prim_step => /=.
+    repeat split => //. apply r_simple. apply rs_local_const; auto.
+  - destruct σ as [[[hs ws] locs] inst].
+    iIntros "!>" (es2 σ2 efs HStep) "!>".
+    destruct σ2 as [[[hs' ws'] locs'] inst'].
+    destruct HStep as (H & -> & ->).
+    iExists _.
+    iFrame. rewrite PeanoNat.Nat.add_0_l.
+    erewrite app_nil_l.
+    only_one_reduction H. all:simplify_eq;iFrame. rewrite Hv. iFrame.
+    1,2,3:rewrite find_first_const// in Hstart.
+Qed.
+
+Lemma wp_return (s: stuckness) (E: coPset) (Φ: val -> iProp Σ) es vs vs0 n f0 f i lh:
+  iris.to_val vs = Some (immV vs0) ->
+  length vs = n ->
+  lfilled i lh (vs ++ [AI_basic BI_return]) es ->
+  WP vs @ s; E {{ v, Φ v ∗ ↪[frame] f0 }} -∗
+  WP [AI_local n f es] @ s; E {{ v, Φ v ∗ ↪[frame] f0 }}%I.
+Proof.
+  iIntros (Hval Hlen Hlf) "HΦ".
+  iApply wp_lift_atomic_step => //=.
+  rewrite wp_unfold /wasm_wp_pre /=.
+  rewrite Hval.
+  iIntros (σ ns κ κs nt) "Hσ !>".
+  assert (const_list vs) as Hcvs; first by apply to_val_const_list in Hval.
+  iSplit.
+  - iPureIntro. destruct s => //=.
+    unfold language.reducible, language.prim_step => /=.
+    exists [], vs, σ, [].
+    destruct σ as [[[hs ws] locs] inst].
+    unfold iris.prim_step => /=.
+    repeat split => //.
+    constructor. econstructor =>//.
+  - destruct σ as [[[hs ws] locs] inst] => //=.
+    iModIntro.
+    iIntros (es1 σ2 efs HStep).
+    iMod "HΦ" as "(HΦ & Hf0)".
+    iModIntro.
+    destruct σ2 as [[[hs' ws'] locs'] inst'] => //=.
+    destruct HStep as [H [-> ->]].
+    only_one_reduction H.
+    + iExists f0.
+      rewrite Hval.
+      iFrame.
+      by iIntros "?".
+    all: assert (lfilled 0 (LH_base vs []) [AI_basic (BI_return)]
+                    (vs ++ [AI_basic (BI_return)]));
+      first (by unfold lfilled, lfill ; rewrite Hcvs ; rewrite app_nil_r);
+    destruct (lfilled_trans _ _ _ _ _ _ _ H Hlf) as [lh' Hfill'] ;
+    eapply lfilled_implies_starts in Hfill' => //= ;
+    unfold first_instr in Hstart ; simpl in Hstart ;
+    unfold first_instr in Hfill' ; rewrite Hfill' in Hstart ;
+    inversion Hstart.
+Qed.
+
+Lemma wp_frame_return (s: stuckness) (E: coPset) (Φ: val -> iProp Σ) vs vs0 n f0 f i lh LI:
+  iris.to_val vs = Some (immV vs0) ->
+  length vs = n ->
+  lfilled i lh (vs ++ [AI_basic BI_return]) LI ->
+  ( WP vs @ s; E {{ v, Φ v ∗ ↪[frame] f0 }}
+  ⊢ WP LI @ s; E FRAME n ; f {{ v, Φ v ∗ ↪[frame] f0 }}).
+Proof.
+  iIntros (Hval Hlen Hlf) "HΦ".
+  by iApply wp_return.
+Qed.
+
+Lemma wp_seq_ctx_frame (s : stuckness) (E : coPset) (Φ Ψ : val -> iProp Σ) (es1 es2 : language.expr wasm_lang) (i : nat) (lh : lholed) (n : nat) (f : frame) (f0 : frame) (f1 : frame) :
+  (↪[frame] f0 ∗
+  (↪[frame] f -∗ WP es1 @ NotStuck; E {{ w, Ψ w ∗ ↪[frame] f1 }}) ∗
+  ∀ w, Ψ w ∗ ↪[frame] f0 -∗ WP (iris.of_val w ++ es2) @ s; E FRAME n ; f1 CTX i; lh {{ v, Φ v }})%I
+  ⊢ WP (es1 ++ es2) @ s; E FRAME n ; f CTX i; lh {{ v, Φ v }}.
+Proof.
+  iLöb as "IH" forall (s E es1 es2 Φ Ψ i lh n f f0 f1).
+{ iIntros "[Hf0 [Hes1 Hes2]]".
+  (* iDestruct (wp_wasm_empty_ctx with "Hes1") as "Hes1". *)
+  iIntros (LI Hfilled).
+  repeat rewrite wp_unfold /wasm_wp_pre /=.
+  (* Base case, when both es1 and es2 are values *)
+  destruct (iris.to_val LI) as [vs|] eqn:Hetov.
+  { destruct vs.
+    { pose proof (filled_is_val_imm _ _ _ _ _ Hetov Hfilled) as
+        [vs [es' [-> [-> [Hconst1 Hconst2]]]]].
+      apply const_list_is_val in Hconst1 as [v1 Hv1].
+      apply const_list_is_val in Hconst2 as [v2 Hv2].
+      edestruct fill_val as [vs12 [Hvs12 Heql]];eauto.
+      assert (Hvs12':=Hvs12).
+      apply to_val_cat in Hvs12' as [-> Hev2].
+      apply iris.of_to_val in Hev2 as <-.
+      iIntros (? ? ? ? ?) "Hσ".
+      destruct σ1 as [[[s0 s1] locs] inst].
+      iDestruct "Hσ" as "(Hfuncs&Htables&Hmems&Hglobals&Hframe&Hlen)".
+      (* We remember the current state now so we can reconstruct it upon return *)
+      iDestruct (ghost_map_lookup with "Hframe Hf0") as %Hlook. rewrite lookup_insert in Hlook. inversion Hlook. subst f0. clear Hlook.
+      (* update the local state to the local state of the inner frame *)
+      iMod (ghost_map_update f with "Hframe Hf0") as "[Hframe Hf0]". rewrite insert_insert.
+      iMod ("Hes1" with "Hf0") as "[HPsi Hf]".
+      (* reconstruct it to its original state for the continuation *)
+      iDestruct (ghost_map_lookup with "Hframe Hf") as %Hlook. rewrite lookup_insert in Hlook. inversion Hlook.
+      iMod (ghost_map_update (Build_frame locs inst) with "Hframe Hf") as "[Hframe Hf0]". rewrite insert_insert.
+      iSpecialize ("Hes2" with "[$HPsi $Hf0]").
+      unfold iris.of_val.
+      rewrite - fmap_app take_drop.
+      rewrite of_val_imm.
+      pose proof (lfilled_swap (iris.of_val (immV vs12)) Hfilled) as [LI' Hfilled'].
+      iSpecialize ("Hes2" $! _ Hfilled').
+      rewrite wp_unfold /wasm_wp_pre /=.
+      iSpecialize ("Hes2" $! (s0,s1,locs,inst) _ _ _ _ with "[$Hfuncs $Htables $Hmems $Hglobals $Hlen $Hframe]").
+      assert (iris.to_val LI' = Some (immV l)) as HLI';[|iFrame].
+      apply lfilled_Ind_Equivalent in Hfilled'. inversion Hfilled';subst.
+      apply to_val_cat_inv;auto. apply to_val_cat_inv;auto. apply iris.to_of_val.
+      apply to_val_immV_inj with (es':=LI') in Hetov as Heq;auto. subst LI.
+      iFrame.
+    }
+    { apply to_val_trap_is_singleton in Hetov. subst.
+      apply lfilled_Ind_Equivalent in Hfilled.
+      inversion Hfilled;subst.
+      2: { exfalso. do 2 destruct vs =>//=. }
+      apply app_eq_singleton in H as [[HH HH']|[HH HH']];subst.
+      { exfalso. destruct es1,es2,es' =>//=. }
+      apply app_eq_singleton in HH' as [[HH HH']|[HH HH']];subst.
+      { apply app_eq_singleton in HH as [[-> ->]|[-> ->]].
+        simpl.
+        all: iIntros (? ? ? ? ?) "Hσ".
+        all: destruct σ1 as [[[s0 s1] locs] inst].
+        all: iDestruct "Hσ" as "(Hfuncs&Htables&Hmems&Hglobals&Hframe&Hlen)".
+        all: iDestruct (ghost_map_lookup with "Hframe Hf0") as %Hlook;rewrite lookup_insert in Hlook;inversion Hlook; clear Hlook.
+        all: iMod (ghost_map_update f with "Hframe Hf0") as "[Hframe Hf0]"; rewrite insert_insert.
+        all: iMod ("Hes1" with "Hf0") as "[HPsi Hf]".
+        all: iDestruct (ghost_map_lookup with "Hframe Hf") as %Hlook; rewrite lookup_insert in Hlook; inversion Hlook.
+        all: iMod (ghost_map_update (Build_frame locs inst) with "Hframe Hf") as "[Hframe Hf0]"; rewrite insert_insert.
+        all: iSpecialize ("Hes2" with "[$HPsi $Hf0]").
+        all: rewrite /=.
+        all: iDestruct (wp_wasm_empty_ctx_frame with "Hes2") as "Hes2".
+        all: rewrite wp_frame_rewrite.
+        all: rewrite wp_unfold /wasm_wp_pre /=.
+        all: by iSpecialize ("Hes2" $! (s0,s1,locs,inst) _ _ _ _ with "[$Hfuncs $Htables $Hmems $Hglobals $Hlen $Hframe]").
+      }
+      { destruct es1,es2 =>//=.
+        iIntros (? ? ? ? ?) "Hσ".
+        destruct σ1 as [[[s0 s1] locs] inst].
+        iDestruct "Hσ" as "(Hfuncs&Htables&Hmems&Hglobals&Hframe&Hlen)".
+        iDestruct (ghost_map_lookup with "Hframe Hf0") as %Hlook;rewrite lookup_insert in Hlook;inversion Hlook;clear Hlook.
+        iMod (ghost_map_update f with "Hframe Hf0") as "[Hframe Hf0]"; rewrite insert_insert.
+        iMod ("Hes1" with "Hf0") as "[HPsi Hf]".
+        iDestruct (ghost_map_lookup with "Hframe Hf") as %Hlook. rewrite lookup_insert in Hlook. inversion Hlook.
+        iMod (ghost_map_update (Build_frame locs inst) with "Hframe Hf") as "[Hframe Hf0]"; rewrite insert_insert.
+        iSpecialize ("Hes2" with "[$HPsi $Hf0]").
+        rewrite /=.
+        iSpecialize ("Hes2" $! [AI_trap] with "[]").
+        { iPureIntro. constructor. }
+        rewrite wp_unfold /wasm_wp_pre /=.
+        by iSpecialize ("Hes2" $! (s0,s1,locs,inst) _ _ _ _ with "[$Hfuncs $Htables $Hmems $Hglobals $Hlen $Hframe]").
+      }
+    }
+  }
+  {
+  (* Ind *)
+  iIntros (σ ns κ κs nt) "Hσ".
+  destruct (iris.to_val es1) as [vs|] eqn:Hes.
+  { apply of_to_val in Hes as <-.
+    destruct σ as [[[s0 s1] locs] inst].
+    iDestruct "Hσ" as "(Hfuncs&Htables&Hmems&Hglobals&Hframe&Hlen)".
+    iDestruct (ghost_map_lookup with "Hframe Hf0") as %Hlook;rewrite lookup_insert in Hlook;inversion Hlook. clear Hlook.
+    iMod (ghost_map_update f with "Hframe Hf0") as "[Hframe Hf0]"; rewrite insert_insert.
+    iMod ("Hes1" with "Hf0") as "[HPsi Hf]".
+    iDestruct (ghost_map_lookup with "Hframe Hf") as %Hlook. rewrite lookup_insert in Hlook. inversion Hlook.
+    iMod (ghost_map_update (Build_frame locs inst) with "Hframe Hf") as "[Hframe Hf0]"; rewrite insert_insert.
+    iSpecialize ("Hes2" with "[$HPsi $Hf0]").
+    iSpecialize ("Hes2" $! _ Hfilled).
+    rewrite wp_unfold /wasm_wp_pre /=.
+    (* rewrite Hetov. *)
+    iSpecialize ("Hes2" $! (s0,s1,locs,inst) ns κ κs nt with "[$]"). subst f.
+    iMod "Hes2" as "[%H1 H2]".
+    iIntros "!>".
+    iSplit.
+    - iPureIntro. by apply H1. 
+    - by iApply "H2".
+  }
+  {
+    destruct σ as [[[s0 s1] locs] inst].
+    iDestruct "Hσ" as "(Hfuncs&Htables&Hmems&Hglobals&Hframe&Hlen)".
+    iDestruct (ghost_map_lookup with "Hframe Hf0") as %Hlook;rewrite lookup_insert in Hlook;inversion Hlook.
+    iMod (ghost_map_update f with "Hframe Hf0") as "[Hframe Hf]"; rewrite insert_insert.
+    iDestruct ("Hes1" with "Hf") as "Hes1".
+    destruct f.
+    iSpecialize ("Hes1" $! (s0,s1,f_locs,f_inst) ns κ κs nt with "[$]").
+    iMod "Hes1" as "[%H1 H2]".
+    iModIntro.
+    iSplit.
+    - iPureIntro.
+      destruct s => //.
+      apply append_reducible with (es2:=es2) in H1;auto.
+      eapply local_frame_lfilled_reducible. apply Hfilled. auto.
+    - iIntros (e2 σ2 efs HStep').
+      destruct σ2 as [[[s2 s3] locs2] inst2].
+      eapply local_frame_lfilled_prim_step_split_reduce_r in HStep' as Heq;[|apply Hfilled|apply H1].
+      destruct Heq as [e' [v'' [i'' [LI' [HStep'' [-> [-> [-> Hfill]]]]]]]].
+      
+      (* eapply lfilled_prim_step_split_reduce_r in HStep' as Heq;[|apply Hfilled|apply H1]. *)
+      (* destruct Heq as [e' [HStep'' Hlfilled']]. *)
+      apply prim_step_obs_efs_empty in HStep'' as Hemp. inversion Hemp;subst;clear Hemp.
+      apply prim_step_obs_efs_empty in HStep' as Hemp. inversion Hemp;subst;clear Hemp.
+      iSpecialize ("H2" $! e' (s2,s3,v'',i'') [] HStep'').
+      iMod "H2".
+      repeat iModIntro.
+      repeat iMod "H2".
+      iDestruct "H2" as (f) "(Hσ & Hf1 & Hes'' & Hefs)".
+      (* iExists f. *)
+      iDestruct "Hσ" as "(Hfuncs&Htables&Hmems&Hglobals&Hframe&Hlen)".
+      iDestruct (ghost_map_lookup with "Hframe Hf1") as %Hlook';rewrite lookup_insert in Hlook';inversion Hlook'.
+      iMod (ghost_map_update (Build_frame locs2 inst2) with "Hframe Hf1") as "[Hframe Hf]"; rewrite insert_insert.
+      iExists _. iFrame.
+      iModIntro.
+      iSplit => //.
+      iIntros "Hf". (* iSpecialize ("Hes''" with "[$]"). *)
+      rewrite -wp_frame_rewrite. iApply ("IH" with "[-]");[|iPureIntro;apply Hfill].
+      iFrame "Hes''". iFrame. Unshelve. all: try apply 0. all: apply [].
+  } } }
+Qed.
+
+(*
+value1
+value2
+value3
+Trap
+expr3
+expr2
+expr1
+
+could reduce to either a Trap directly, or 
+value1
+Trap
+expr1,
+
+But ultimately they reduce to a single Trap.
+*)
+
+(*
+Lemma wp_trap s E es Φ:
+  WP @ s; E ([AI_trap] ++ es) {{ w, Φ w }} ⊢
+  |={E}=> Φ trapV.
+Proof.
+  rewrite wp_unfold/ wp_pre.
+Admitted.
+ *)
+
+(* behaviour of seq might be a bit unusual due to how reductions work. *)
+(* Note that the sequence wp is also true without the premise that Ψ doesn't trap, but it is very tricky to prove that version. The following is the fault-avoiding version.*)
+Lemma wp_seq (s : stuckness) (E : coPset) (Φ Ψ : val -> iProp Σ) (es1 es2 : language.expr wasm_lang) :
+  (¬ Ψ trapV) ∗ 
+  (WP es1 @ s; E {{ w, Ψ w }} ∗
+  ∀ w, Ψ w -∗ WP (iris.of_val w ++ es2) @ s; E {{ v, Φ v }})%I
+  ⊢ WP (es1 ++ es2) @ s; E {{ v, Φ v }}.
+Proof.
+  iLöb as "IH" forall (s E es1 es2 Φ Ψ).
+  iIntros "(Hntrap & Hes1 & Hes2)".
+  repeat rewrite wp_unfold /wasm_wp_pre /=.
+  (* Base case, when both es1 and es2 are values *)
+  destruct (iris.to_val (es1 ++ es2)) as [vs|] eqn:Hetov.
+  {
+    destruct vs.
+    {
+      apply to_val_cat in Hetov as [-> Hev2].
+      apply iris.of_to_val in Hev2 as <-.
+      iMod "Hes1".
+      iSpecialize ("Hes2" with "Hes1").
+      unfold iris.of_val.
+      rewrite - fmap_app take_drop.
+      rewrite of_val_imm.
+      rewrite wp_unfold /wasm_wp_pre /=.
+      rewrite of_val_imm iris.to_of_val.
+      by iAssumption.
+    }
+    {
+      apply to_val_trap_is_singleton in Hetov.
+      apply app_eq_singleton in Hetov as [[-> ->]|[-> ->]].
+      all:iMod "Hes1".
+      all: iSpecialize ("Hes2" with "Hes1").
+      all:rewrite /=.
+      all:by rewrite wp_unfold /wasm_wp_pre /=. 
+    }
+  }
+  (* Ind *)
+  iIntros (σ ns κ κs nt) "Hσ".
+  destruct (iris.to_val es1) as [vs|] eqn:Hes.
+  { apply of_to_val in Hes as <-.
+    iMod "Hes1".
+    iSpecialize ("Hes2" with "Hes1").
+    rewrite wp_unfold /wasm_wp_pre /=.
+    rewrite Hetov.
+    iSpecialize ("Hes2" $! σ ns κ κs nt with "[$]").
+    iMod "Hes2" as "[%H1 H2]".
+    iIntros "!>".
+    iSplit.
+    - iPureIntro. by apply H1. 
+    - by iApply "H2".
+  }
+  {
+    iSpecialize ("Hes1" $! σ ns κ κs nt with "[$]").
+    iMod "Hes1" as "[%H1 H2]".
+    iModIntro.
+    iSplit.
+    - iPureIntro.
+      destruct s => //.
+      by apply append_reducible.
+    - iIntros (e2 σ2 efs HStep).
+      assert (κ = [] /\ efs = []) as [-> ->]; first by apply prim_step_obs_efs_empty in HStep; inversion HStep.
+      apply prim_step_split_reduce_r in HStep; last by [].
+      destruct HStep as [[es'' [-> HStep]] | [n [m [lh [Hlf1 [Hlf2 ->]]]]]].
+      + iSpecialize ("H2" $! es'' σ2 [] HStep).
+        iMod "H2".
+        repeat iModIntro.
+        repeat iMod "H2".
+        iModIntro.
+        destruct σ2 as [[[??] ?]?].
+        iDestruct "H2" as (f1) "(Hσ & Hf1 & Hes'' & Hefs)".
+        iExists f1.
+        iFrame.
+        iIntros "?"; iSpecialize ("Hes''" with "[$]").
+        iApply "IH".
+        by iFrame. 
+      + move/lfilledP in Hlf1.
+        inversion Hlf1; subst; clear Hlf1.
+        assert (iris.prim_step es1 σ [] [AI_trap] σ []) as HStep2.
+        { unfold iris.prim_step.
+          destruct σ as [[[??]?]?].
+          repeat split => //.
+          apply r_simple; eapply rs_trap => //.
+          move => HContra; subst.
+          by destruct n.
+        }
+        iSpecialize ("H2" $! [AI_trap] σ [] HStep2).
+        iMod "H2".
+        repeat iModIntro.
+        repeat iMod "H2".
+        destruct σ as [[[??] ?]?].
+        iDestruct "H2" as (f1) "(Hσ & Hf1 & Hes'' & Hefs)".
+        iExists f1.
+        iModIntro.
+        iFrame.
+        iIntros "?"; iSpecialize ("Hes''" with "[$]").
+        replace [AI_trap] with (iris.of_val trapV) => //.
+        repeat rewrite wp_unfold /wasm_wp_pre /=.
+        destruct (iris.to_val (take n es1 ++ AI_trap :: drop m (es1 ++ es2))%SEQ) eqn:Hx.
+        * iMod "Hes''".
+          by iSpecialize ("Hntrap" with "Hes''").
+        * iIntros (?????) "?".
+          iMod "Hes''".
+          by iSpecialize ("Hntrap" with "Hes''").
+  }
+Qed.
+
+Lemma wp_val (s : stuckness) (E : coPset) (Φ : val -> iProp Σ) (v0 : value) (es : language.expr wasm_lang) :
+  (* Like for wp_seq, this lemma is true without the trap condition, but would
+     be problematic to prove without it. *)
+  ((¬ Φ trapV) ∗
+  WP es @ NotStuck ; E {{ v, (Φ (val_combine (immV [v0]) v))  }}
+  ⊢ WP ((AI_basic (BI_const v0)) :: es) @ s ; E {{ v, Φ v }})%I.
+Proof.
+  (* This also needs an iLob. *)
+  iLöb as "IH" forall (v0 es Φ).
+  iIntros "(Hntrap & H)".
+  repeat rewrite wp_unfold /wasm_wp_pre /=.
+  destruct (iris.to_val es) as [vs|] eqn:Hes.
+  {
+    destruct vs; first by apply of_to_val in Hes as <-.
+    iIntros (?????) "?".
+    iMod "H".
+    by iSpecialize ("Hntrap" with "H").
+  }
+  {
+    iIntros (σ ns κ κs nt) "Hσ".
+    iSpecialize ("H" $! σ ns κ κs nt with "[$]").
+    iMod "H".
+    iModIntro.
+    iDestruct "H" as "(%H1 & H)".
+    iSplit.
+    - iPureIntro.
+      destruct s => //=.
+      rewrite - cat1s.
+      by eapply prepend_reducible; eauto.
+    - iIntros (es2 σ2 efs HStep).
+      rewrite -cat1s in HStep.
+      eapply reduce_ves in H1; last by apply HStep.
+      assert (κ = [] /\ efs = []) as [-> ->]; first by apply prim_step_obs_efs_empty in HStep; inversion HStep.
+      destruct H1 as [[-> HStep2] | [lh1 [lh2 [Hlf1 [Hlf2 ->]]]]].
+      + iSpecialize ("H" $! (drop 1 es2) σ2 [] HStep2).
+        iMod "H".
+        repeat iModIntro.
+        repeat iMod "H".
+        iModIntro.
+        iDestruct "H" as (f1) "(Hσ & Hf1 & Hes & Hefs)".
+        iSimpl.
+        iExists f1.
+        iFrame.
+        iSplit => //.
+        iIntros "?"; iSpecialize ("Hes" with "[$]").
+        iApply "IH".
+        by iFrame.
+      + move/lfilledP in Hlf1.
+        inversion Hlf1; subst; clear Hlf1.
+        move/lfilledP in Hlf2.
+        inversion Hlf2; subst; clear Hlf2.
+        assert (iris.prim_step (vs0 ++ [AI_trap] ++ es'0) σ2 [] [AI_trap] σ2 []) as HStep2.
+        { unfold iris.prim_step.
+          destruct σ2 as [[[??]?]?].
+          repeat split => //.
+          apply r_simple; eapply rs_trap => //.
+          - move => HContra.
+            by replace (vs0 ++ [AI_trap] ++ es'0)%SEQ with [AI_trap] in Hes.
+          - apply/lfilledP.
+            by apply LfilledBase.
+        }
+        iSpecialize ("H" $! [AI_trap] σ2 [] HStep2).
+        iMod "H".
+        repeat iModIntro.
+        repeat iMod "H".
+        iDestruct "H" as (f1) "(Hσ & Hf1 & Hes & Hefs)".
+        iExists f1.
+        iFrame.
+        iModIntro.
+        iSplit => //.
+        iIntros "?"; iSpecialize ("Hes" with "[$]").
+        repeat rewrite wp_unfold /wasm_wp_pre /=.
+        destruct (iris.to_val (vs ++ AI_trap :: es')%SEQ) eqn:Hx.
+        * iMod "Hes".
+          by iSpecialize ("Hntrap" with "Hes").
+        * iIntros (?????) "?".
+          iMod "Hes".
+          by iSpecialize ("Hntrap" with "Hes").
+  }
+Qed.
+  
+Lemma wp_val_app' (s : stuckness) (E : coPset) (Φ : val -> iProp Σ) vs (es : language.expr wasm_lang) :
+  (* □ is required here -- this knowledge needs to be persistent instead of 
+     one-off. *)
+  (□ (¬ Φ trapV )) ∗
+  WP es @ NotStuck ; E {{ v, (Φ (val_combine (immV vs) v)) }}%I
+  ⊢ WP ((v_to_e_list vs) ++ es) @ s ; E {{ v, Φ v }}%I.
+
+Proof.
+  iInduction vs as [|c vs] "IH" forall (Φ s E es).
+  { simpl.
+    iIntros "(#Hntrap & HWP)".
+    destruct s.
+    2: iApply wp_stuck_weaken.
+    all: iApply (wp_wand with "HWP").
+    all: iIntros (v).
+    all: destruct v => /=.
+    all: iIntros "HΦ" => //.
+  }
+  { iIntros "(#Hntrap & HWP)".
+    iSimpl.
+    iApply wp_val.
+    iSplitR => //.
+    iApply "IH" => //=.
+    iSplit => //.
+    iApply (wp_mono with "HWP").
+    iIntros (vs') "HΦ".
+    iSimpl. destruct vs';auto.
+  }
+Qed.
+  
+Lemma wp_val_app (s : stuckness) (E : coPset) (Φ : val -> iProp Σ) vs v' (es : language.expr wasm_lang) :
+  iris.to_val vs = Some (immV v') ->
+  (□ (¬ Φ trapV )) ∗
+  WP es @ NotStuck ; E {{ v, (Φ (val_combine (immV v') v)) }}%I
+  ⊢ WP (vs ++ es) @ s ; E {{ v, Φ v }}%I.
+Proof.
+  iIntros "%Hves [#Hntrap Hwp]".
+  apply iris.of_to_val in Hves; subst.
+  iApply wp_val_app'.
+  by iFrame.
+Qed.
+                                  
+(* Trying to resolve the problem by naively not allowing any consumption of ↪ in
+   the WP premises.
+
+   However, we then cannot connect the resulting frame after executing es1 to 
+   that at the start of es2: the only way to achieve that is to have a 
+   ↪[frame] in the post condition of es1; but to prove any WP with that post
+   condition, we need to provide a ↪[frame] to its precondition as well; 
+   so we will need two copies of the same ↪ to prove any WP, rendering the 
+   spec useless.
+
+   What we need in the post condition is some predicate like ↪ which gives
+   us the knowledge of the new frame, but does not actually assert any 
+   ownership -- in some sense, we need to be able to assert 0 ownership of 
+   something while still asserting the knowledge of that value. This seems to
+   be a weird feature to ask for, however.
+ *)
+(* Upd: THIS IS DONE!!!!
+        Note how the post condition successfully prevents the leakage of any
+        frame resources from the inner to the outer frame via Ψ -- the outer 
+        frame predicate remains unchanged despite that it could undergo 
+        arbitrary changes inside the frames. *)
+Lemma wp_frame_seq es1 es2 n (f0 f f': frame) E Ψ Φ:
+  ( ↪[frame] f0) -∗
+  (¬ (Ψ trapV)) -∗
+  ((↪[frame] f) -∗ WP es1 @ NotStuck; E {{ v, ↪[frame] f' ∗ Ψ v }}) -∗
+  (∀ w, ↪[frame] f0 -∗ (Ψ w) -∗ WP (iris.of_val w ++ es2) @ NotStuck; E FRAME n; f' {{ v, Φ v ∗ ↪[frame] f0 }}) -∗
+  (WP (es1 ++ es2) @ NotStuck; E FRAME n ; f {{ v, Φ v ∗ ↪[frame]f0 }}).
+(* WP [AI_local n f (es1 ++ es2)] @ NotStuck; E {{ v, Φ v }} *)
+Proof.
+  iLöb as "IH" forall (f0 f f' E es1 es2 Ψ Φ n).
+  iIntros "Hf0 Hntrap Hwp1 Hwp2".
+  unfold wp_wasm_frame.
+  repeat rewrite wp_unfold /wasm_wp_pre /=.
+  destruct (iris.to_val es1) as [vs|] eqn:Hetov.
+  
+  { (* when es1 is a value, the post condition of the first wp needs to
+       provide enough information for the second wp to work. *)
+    iIntros (σ ns κ κs nt) "Hσ".
+    destruct σ as [[[hs ws] locs] inst].
+    iDestruct "Hσ" as "(Hfunc&Ht&Hm&Hg& Hframe & Hmemlen)".
+    (* We must always remember to link the frame predicate to the state interp:
+       else we lose their relationship when we update the state later. *)
+    iDestruct (ghost_map_lookup with "Hframe Hf0") as "%Hf".
+    rewrite lookup_insert in Hf.
+    inversion Hf; subst; clear Hf.
+    iMod (ghost_map_update with "Hframe Hf0") as "(Hframe & Hf0)".
+    instantiate (1 := f).
+    iSpecialize ("Hwp1" with "[$]").
+    iMod "Hwp1" as "(Hf' & HΨ)".
+    (* Again, must remember to link f' to the state interp here *)
+    iDestruct (ghost_map_lookup with "Hframe Hf'") as "%Hf'".
+    rewrite lookup_insert in Hf'.
+    inversion Hf'; subst; clear Hf'.
+    iMod (ghost_map_update with "Hframe Hf'") as "(Hframe & Hf')".
+    instantiate (1 := (Build_frame locs inst)).
+    iSpecialize ("Hwp2" $! vs with "[$] [$]").
+    rewrite wp_unfold /wasm_wp_pre /=.
+    repeat rewrite insert_insert.
+    iSpecialize ("Hwp2" $! (hs, ws, locs, inst) ns κ κs nt
+                   with "[$Hfunc $Ht $Hm $Hg Hframe $Hmemlen]"); first by destruct f'.
+    iMod "Hwp2" as "(%Hreducible & Hwp2)".
+    iModIntro.
+    apply of_to_val in Hetov as <-.
+    by iSplit.
+  }
+  { 
+    iIntros (σ ns κ κs nt) "Hσ".
+    destruct σ as [[[hs ws] locs] inst].
+    iDestruct "Hσ" as "(Hf & Ht & Hm & Hg & Hframe & Hmemlen)".
+    iDestruct (ghost_map_lookup with "Hframe Hf0") as "%Hf0".
+    rewrite lookup_insert in Hf0.
+    inversion Hf0; subst; clear Hf0.
+    iMod (ghost_map_update with "Hframe Hf0") as "(Hframe & Hfx)".
+    instantiate (1 := f).
+    iSpecialize ("Hwp1" with "Hfx").
+    iSpecialize ("Hwp1" $! (hs, ws, f.(f_locs), f.(f_inst)) ns [] κs nt).
+    rewrite insert_insert.
+    iSpecialize ("Hwp1" with "[$Hf $Ht $Hm $Hg $Hmemlen Hframe]"); first by destruct f => /=.
+    iMod "Hwp1" as "(%Hreducible & Hwp1)".
+    iModIntro.
+    iSplit.
+    { (* reducibility of seq within AI_local. *)
+      iPureIntro.
+      unfold reducible, language.reducible, language.prim_step in *.
+      destruct Hreducible as [κ' [es'[σ'[efs HStep]]]].
+      destruct σ' as [[[hs' ws'] locs'] inst'].
+      exists κ', [AI_local n (Build_frame locs' inst') (es' ++ es2)], (hs', ws', locs, inst), [].
+      simpl in *.
+      destruct HStep as [Hreduce [-> ->]].
+      repeat split => //.
+      apply r_local.
+      destruct f.
+      by apply r_elimr.
+    }
+    iIntros (es' σ' efs HStep).
+    destruct σ' as [[[hs' ws'] locs'] inst'].
+
+    inversion HStep as [Hreduce [-> ->]].
+    apply AI_local_reduce in Hreduce as [f'' [es'' [Hf0 [-> Hreduce]]]].
+    inversion Hf0; subst; clear Hf0.
+    apply reduce_tmp in Hreduce as [es1' [Hreduce' ->]] => //.
+    iSpecialize ("Hwp1" $! es1' (hs', ws', f''.(f_locs), f''.(f_inst)) [] with "[%]"); first ((repeat split); by destruct f, f'') => //=.
+  
+    (* We can't eliminate all the modalities -- one fupd needs to remain for us
+       to update the frame back. But the masks in Hwp1 can be stripped *)
+    iMod "Hwp1".
+    do 2 iModIntro.
+    iMod "Hwp1".
+    iModIntro.
+    iMod "Hwp1".
+
+    iDestruct "Hwp1" as (f1) "((?&?&?&?& Hframe &?) & Hf1 & Hwp1 & ?)".
+
+    (* Establish the relationship between f1 and f'' the cell gets consumed. This
+       is also the reason that we can have an arbitrary existential in the 
+       definition of the weakest precondition fixpoint. *)
+    iDestruct (ghost_map_lookup with "Hframe Hf1") as "%Hf".
+    rewrite lookup_insert in Hf.
+    inversion Hf; subst; clear Hf.
+    
+    
+    (* Now we do have the ↪; modify the ghost_map back to f0 *)
+    iMod (ghost_map_update with "Hframe Hf1") as "(Hframe & Hf1)".
+    instantiate (1 := Build_frame locs' inst').
+    rewrite insert_insert.
+    iExists (Build_frame locs' inst').
+  
+    iModIntro.
+    iFrame => /=.
+
+    iIntros "Hf1".
+    
+    iApply ("IH" with "[Hf1] [Hntrap] [Hwp1]") => //.
+    destruct f''.
+    iIntros "?"; iSpecialize ("Hwp1" with "[$]").
+    by iAssumption.
+  }
+(*
+   The key that enables the above to be proved is the modification of wp: instead
+   of only knowing that a frame predicate exists at the end, we now know that
+   it exists at each step. Note that this could not have worked without changing
+   the wp: the statement that there is always a frame ownership is not an
+   universal property of Iris, but a property of the Wasm semantics instead.
+   As a result, we need this specific version of wp to prove this result.
+   Also, we need to prove that every reduction respects this preservation of 
+   the existence of a frame ownership.
+ *)
+Qed.
