theories/iris_wp_def.v
@@ -1,0 +1,461 @@
+From mathcomp Require Import ssreflect eqtype seq ssrbool.
+From iris.program_logic Require Import language.
+From iris.proofmode Require Import base tactics classes.
+From iris.base_logic Require Export gen_heap ghost_map proph_map.
+From iris.base_logic.lib Require Export fancy_updates.
+From iris.bi Require Export weakestpre.
+Require Export iris iris_locations iris_properties iris_atomicity stdpp_aux.
+Require Export datatypes host operations properties opsem.
+
+Import uPred.
+
+Set Default Proof Using "Type". (* what is this? *)
+
+Close Scope byte_scope.
+
+Let expr := iris.expr.
+Let val := iris.val.
+Let to_val := iris.to_val.
+
+(* Defining a Wasm-specific WP with frame existence *)
+
+Import DummyHosts.
+  (*
+Let reduce := @reduce host_function host_instance.
+*)
+
+Canonical Structure wasm_lang := Language wasm_mixin.
+ 
+Let reducible := @reducible wasm_lang.
+
+Class irisG (Σ : gFunctors) := IrisG {
+  iris_invG :> invG Σ;
+
+  (** The state interpretation is an invariant that should hold in
+  between each step of reduction. Here [Λstate] is the global state,
+  the first [nat] is the number of steps already performed by the
+  program, [list Λobservation] are the remaining observations, and the
+  last [nat] is the number of forked-off threads (not the total number
+  of threads, which is one higher because there is always a main
+  thread). *)
+  state_interp : state → nat → list (observation) → nat → iProp Σ;
+
+  (** A fixed postcondition for any forked-off thread. For most languages, e.g.
+  heap_lang, this will simply be [True]. However, it is useful if one wants to
+  keep track of resources precisely, as in e.g. Iron. *)
+  fork_post : val → iProp Σ;
+
+  (** Number of additional logical steps (i.e., later modality in the
+  definition of WP) per physical step, depending on the physical steps
+  counter. In addition to these steps, the definition of WP adds one
+  extra later per physical step to make sure that there is at least
+  one later for each physical step. *)
+  num_laters_per_step : nat → nat;
+
+  (** When performing pure steps, the state interpretation needs to be
+  adapted for the change in the [ns] parameter.
+
+  Note that we use an empty-mask fancy update here. We could also use
+  a basic update or a bare magic wand, the expressiveness of the
+  framework would be the same. If we removed the modality here, then
+  the client would have to include the modality it needs as part of
+  the definition of [state_interp]. Since adding the modality as part
+  of the definition [state_interp_mono] does not significantly
+  complicate the formalization in Iris, we prefer simplifying the
+  client. *)
+  state_interp_mono σ ns κs nt:
+    state_interp σ ns κs nt ={∅}=∗ state_interp σ (S ns) κs nt
+}.
+Global Opaque iris_invG.
+
+(* TODO: change the fields to use actual sensible names *)
+Class wfuncG Σ := WFuncG {
+  func_invG :> invG Σ;
+  func_gen_hsG :> gen_heapG N function_closure Σ;
+}.
+
+Class wtabG Σ := WTabG {
+  tab_gen_hsG :> gen_heapG (N*N) funcelem Σ;
+}.
+
+Class wmemG Σ := WMemG {
+  mem_gen_hsG :> gen_heapG (N*N) byte Σ;
+}.
+
+Class wmemsizeG Σ := WMemsizeG {
+  memsize_gen_hsG :> gen_heapG N N Σ;
+}.
+
+Class wglobG Σ := WGlobG {
+  glob_gen_hsG :> gen_heapG N global Σ;
+}.
+
+Class wframeG Σ := WFrameG {
+  locs_gen_hsG :> ghost_mapG Σ unit frame;
+}.
+
+Definition frameGName : positive := 10%positive.
+
+Definition proph_id := positive. (* ??? *)
+
+
+Instance eqdecision_frame: EqDecision frame.
+Proof. decidable_equality. Qed.
+
+(* TODO: Global Instance doesn't seem to actually make this global... *)
+Global Instance heapG_irisG `{!wfuncG Σ, !wtabG Σ, !wmemG Σ, wmemsizeG Σ, !wglobG Σ, !wframeG Σ} : irisG Σ := {
+  iris_invG := func_invG; (* ??? *)
+  state_interp σ _ κs _ :=
+    let: (_, s, locs, inst) := σ in
+     ((gen_heap_interp (gmap_of_list s.(s_funcs))) ∗
+      (gen_heap_interp (gmap_of_table s.(s_tables))) ∗
+      (gen_heap_interp (gmap_of_memory s.(s_mems))) ∗
+      (gen_heap_interp (gmap_of_list s.(s_globals))) ∗
+      (ghost_map_auth frameGName 1 (<[ tt := Build_frame locs inst ]> ∅)) ∗ 
+      (gen_heap_interp (gmap_of_list (fmap mem_length s.(s_mems))))
+      
+    )%I;
+    num_laters_per_step _ := 0;
+    fork_post _ := True%I;
+    state_interp_mono _ _ _ _ := fupd_intro _ _
+}.
+
+
+(* Resource ownerships *)
+Notation "n ↦[wf]{ q } v" := (mapsto (L:=N) (V:=function_closure) n q v%V)
+                           (at level 20, q at level 5, format "n ↦[wf]{ q } v") : bi_scope.
+Notation "n ↦[wf] v" := (mapsto (L:=N) (V:=function_closure) n (DfracOwn 1) v%V)
+                      (at level 20, format "n ↦[wf] v") : bi_scope.
+Notation "n ↦[wt]{ q } [ i ] v" := (mapsto (L:=N*N) (V:=funcelem) (n, i) q v%V)
+                           (at level 20, q at level 5, format "n ↦[wt]{ q } [ i ] v") : bi_scope.
+Notation "n ↦[wt][ i ] v" := (mapsto (L:=N*N) (V:=funcelem) (n, i) (DfracOwn 1) v%V)
+                      (at level 20, format "n ↦[wt][ i ] v") : bi_scope.
+Notation "n ↦[wm]{ q } [ i ] v" := (mapsto (L:=N*N) (V:=byte) (n, i) q v%V)
+                           (at level 20, q at level 5, format "n ↦[wm]{ q } [ i ] v") : bi_scope.
+Notation "n ↦[wm][ i ] v" := (mapsto (L:=N*N) (V:=byte) (n, i) (DfracOwn 1) v% V)
+                           (at level 20, format "n ↦[wm][ i ] v") : bi_scope.
+Notation "n ↦[wmlength] v" := (mapsto (L:=N) (V:=N) n (DfracOwn 1) v% V)
+                           (at level 20, format "n ↦[wmlength] v") : bi_scope.
+Notation "n ↦[wg]{ q } v" := (mapsto (L:=N) (V:=global) n q v%V)
+                           (at level 20, q at level 5, format "n ↦[wg]{ q } v").
+Notation "n ↦[wg] v" := (mapsto (L:=N) (V:=global) n (DfracOwn 1) v%V)
+                      (at level 20, format "n ↦[wg] v") .
+Notation " ↪[frame]{ q } v" := (ghost_map_elem frameGName tt q v%V)
+                           (at level 20, q at level 5, format " ↪[frame]{ q } v") .
+Notation " ↪[frame] v" := (ghost_map_elem frameGName tt (DfracOwn 1) v%V)
+                           (at level 20, format " ↪[frame] v").
+
+
+
+Section Wasm_wp.
+  
+Context `{!wfuncG Σ, !wtabG Σ, !wmemG Σ, !wmemsizeG Σ, !wglobG Σ, !wframeG Σ}.
+
+Definition wasm_wp_pre (s : stuckness)
+    (wp : coPset -d> expr -d> (val -d> iPropO Σ) -d> iPropO Σ) :
+  coPset -d> expr -d> (val -d> iPropO Σ) -d> iPropO Σ := λ E e1 Φ,
+  (match iris.to_val e1 with
+  | Some v => |={E}=> Φ v
+  | None => ∀ σ1 ns κ κs nt,
+     (state_interp σ1 ns (κ ++ κs) nt) ={E,∅}=∗
+       ⌜if s is NotStuck then reducible e1 σ1 else True⌝ ∗
+       ∀ e2 σ2 efs, ⌜prim_step e1 σ1 κ e2 σ2 efs⌝
+         ={∅}▷=∗^(S $ num_laters_per_step ns) |={∅,E}=>
+     ∃ f, state_interp σ2 (S ns) κs (length efs + nt) ∗
+         (* Although it's an existential, we know what it must be. *)  
+         ↪[frame] f ∗
+         (↪[frame] f -∗ wp E e2 Φ) ∗
+         [∗ list] i ↦ ef ∈ efs, wp ⊤ ef fork_post
+end)%I.
+
+Global Instance wasm_wp_pre_contractive s: Contractive (wasm_wp_pre s).
+Proof.
+  rewrite /wasm_wp_pre /= => n wp wp' Hwp E e1 Φ.
+  do 24 (f_contractive || f_equiv).
+  (* FIXME : simplify this proof once we have a good definition and a
+     proper instance for step_fupdN. *)
+  induction num_laters_per_step as [|k IH]; simpl => //.
+  repeat (f_contractive || f_equiv); apply Hwp.
+Qed.
+
+Global Instance wasm_wp_def : Wp wasm_lang (iProp Σ) stuckness :=
+  λ (s: stuckness), fixpoint (wasm_wp_pre s).
+
+(* Seal is a mechanism that stdpp uses to avoid definitions being automatically
+   unfolded. *)
+Definition wasm_wp_aux : seal (@wasm_wp_def). Proof. by exists wasm_wp_def. Qed.
+Definition wasm_wp' := wasm_wp_aux.(unseal).
+Global Arguments wasm_wp' {Λ Σ _}.
+Global Existing Instance wasm_wp'.
+Lemma wasm_wp_eq: wp = @wasm_wp_def.
+Proof. rewrite -wasm_wp_aux.(seal_eq) //. Qed.
+
+(* Reprove some useful auxiliary lemmas *)
+Lemma wp_unfold s E e Φ :
+  WP e @ s; E {{ Φ }} ⊣⊢ wasm_wp_pre s (wp (PROP:=iProp Σ) s) E e Φ.
+Proof. rewrite wasm_wp_eq. apply (fixpoint_unfold (wasm_wp_pre s)). Qed.
+
+Lemma wp_value_fupd' s E Φ v : WP of_val v @ s; E {{ Φ }} ⊣⊢ |={E}=> Φ v.
+Proof. rewrite wp_unfold /wasm_wp_pre to_of_val. auto. Qed.
+
+Lemma wp_strong_mono s1 s2 E1 E2 e Φ Ψ :
+  s1 ⊑ s2 → E1 ⊆ E2 ->
+  WP e @ s1; E1 {{ Φ }} -∗ (∀ v, Φ v ={E2}=∗ Ψ v) -∗ WP e @ s2; E2 {{ Ψ }}.
+Proof.
+  iIntros (? HE) "H HΦ". iLöb as "IH" forall (e E1 E2 HE Φ Ψ).
+  rewrite !wp_unfold /wasm_wp_pre.
+  destruct (iris.to_val e) as [v|] eqn:?.
+  { iApply ("HΦ" with "[> -]"). by iApply (fupd_mask_mono E1 _). }
+  iIntros (σ1 ns κ κs nt) "Hσ".
+  iMod (fupd_mask_subseteq E1) as "Hclose"; first done.
+  iMod ("H" with "[$]") as "[% H]".
+  iModIntro. iSplit; [by destruct s1, s2|]. iIntros (e2 σ2 efs Hstep).
+  iMod ("H" with "[//]") as "H". iIntros "!> !>".
+  iMod "H".
+  simpl.
+  iMod "H" as (f1) "(Hσ & Hf1 & H & Hefs)".
+  iMod "Hclose" as "_".
+  iApply fupd_mask_intro; first by solve_ndisj.
+  iIntros "Hmask".
+  iMod "Hmask". iModIntro. iExists f1. iFrame. iSplitR "Hefs".
+  - iIntros "Hf1".
+    iSpecialize ("H" with "Hf1").                             
+    by iApply ("IH" with "[//] H HΦ").
+  - iApply (big_sepL_impl with "Hefs"); iIntros "!>" (k ef _).
+    iIntros "H". iApply ("IH" with "[] H"); auto.
+Qed.
+
+Lemma wp_mono s E e Φ Ψ : (∀ v, Φ v ⊢ Ψ v) → WP e @ s; E {{ Φ }} ⊢ WP e @ s; E {{ Ψ }}.
+Proof.
+  iIntros (HΦ) "H"; iApply (wp_strong_mono with "H"); auto.
+  iIntros (v) "?". by iApply HΦ.
+Qed.
+Lemma wp_stuck_mono s1 s2 E e Φ :
+  s1 ⊑ s2 → WP e @ s1; E {{ Φ }} ⊢ WP e @ s2; E {{ Φ }}.
+Proof. iIntros (?) "H". iApply (wp_strong_mono with "H"); auto. Qed.
+Lemma wp_stuck_weaken s E e Φ :
+  WP e @ s; E {{ Φ }} ⊢ WP e @ E ?{{ Φ }}.
+Proof. apply wp_stuck_mono. by destruct s. Qed.
+Lemma wp_mask_mono s E1 E2 e Φ : E1 ⊆ E2 → WP e @ s; E1 {{ Φ }} ⊢ WP e @ s; E2 {{ Φ }}.
+Proof. iIntros (?) "H"; iApply (wp_strong_mono with "H"); auto. Qed.
+Global Instance wp_mono' s E e :
+  Proper (pointwise_relation _ (⊢) ==> (⊢)) (wp (PROP:=iProp Σ) s E e).
+Proof. by intros Φ Φ' ?; apply wp_mono. Qed.
+Global Instance wp_flip_mono' s E e :
+  Proper (pointwise_relation _ (flip (⊢)) ==> (flip (⊢))) (wp (PROP:=iProp Σ) s E e).
+Proof. by intros Φ Φ' ?; apply wp_mono. Qed.
+
+Lemma wp_value_fupd s E Φ e v : IntoVal e v → WP e @ s; E {{ Φ }} ⊣⊢ |={E}=> Φ v.
+Proof. intros <-. by apply wp_value_fupd'. Qed.
+Lemma wp_value' s E Φ v : Φ v ⊢ WP (of_val v) @ s; E {{ Φ }}.
+Proof. rewrite wp_value_fupd'. auto. Qed.
+Lemma wp_value s E Φ e v : IntoVal e v → Φ v ⊢ WP e @ s; E {{ Φ }}.
+Proof. intros <-. apply wp_value'. Qed.
+
+Lemma wp_wand s E e Φ Ψ :
+  WP e @ s; E {{ Φ }} -∗ (∀ v, Φ v -∗ Ψ v) -∗ WP e @ s; E {{ Ψ }}.
+Proof.
+  iIntros "Hwp H". iApply (wp_strong_mono with "Hwp"); auto.
+  iIntros (?) "?". by iApply "H".
+Qed.
+Lemma wp_wand_l s E e Φ Ψ :
+  (∀ v, Φ v -∗ Ψ v) ∗ WP e @ s; E {{ Φ }} ⊢ WP e @ s; E {{ Ψ }}.
+Proof. iIntros "[H Hwp]". iApply (wp_wand with "Hwp H"). Qed.
+Lemma wp_wand_r s E e Φ Ψ :
+  WP e @ s; E {{ Φ }} ∗ (∀ v, Φ v -∗ Ψ v) ⊢ WP e @ s; E {{ Ψ }}.
+Proof. iIntros "[Hwp H]". iApply (wp_wand with "Hwp H"). Qed.
+Lemma wp_frame_wand_l s E e Q Φ :
+  Q ∗ WP e @ s; E {{ v, Q -∗ Φ v }} -∗ WP e @ s; E {{ Φ }}.
+Proof.
+  iIntros "[HQ HWP]". iApply (wp_wand with "HWP").
+  iIntros (v) "HΦ". by iApply "HΦ".
+Qed.
+
+(* Some lifting lemmas restated and reproved *)
+Lemma wp_lift_step_fupd s E Φ e1 :
+  iris.to_val e1 = None →
+  (∀ σ1 ns κ κs nt, state_interp σ1 ns (κ ++ κs) nt ={E,∅}=∗
+    ⌜if s is NotStuck then reducible e1 σ1 else True⌝ ∗
+    ∀ e2 σ2 efs, ⌜prim_step e1 σ1 κ e2 σ2 efs⌝ ={∅}=∗ ▷ |={∅,E}=>
+   ∃ f, state_interp σ2 (S ns) κs (length efs + nt) ∗
+      ↪[frame] f ∗
+      (↪[frame] f -∗ WP e2 @ s; E {{ Φ }}) ∗
+      [∗ list] ef ∈ efs, WP ef @ s; ⊤ {{ fork_post }})
+    ⊢ WP e1 @ s; E {{ Φ }}.
+Proof.
+  (* Somehow, this lemma can no longer be automatically proved in one unfold. *)
+  rewrite wp_unfold /wasm_wp_pre=>->. iIntros "H".
+  iIntros (σ ns κ κs nt) "Hσ".
+  iSpecialize ("H" $! σ ns κ κs nt with "[$]").
+  iMod "H" as "(%Hred & H)".
+  iModIntro.
+  iSplit => //.
+  iIntros (es' σ' efs HStep).
+  iSpecialize ("H" $! es' σ' efs with "[% //]").
+  repeat iMod "H".
+  repeat iModIntro.
+  simpl.
+  iMod "H" as (f) "H".
+  iModIntro.
+  by iExists f.
+Qed.
+
+Lemma wp_lift_stuck E Φ e :
+  iris.to_val e = None →
+  (∀ ns σ κs nt, state_interp σ ns κs nt ={E,∅}=∗ ⌜stuck e σ⌝)
+  ⊢ WP e @ E ?{{ Φ }}.
+Proof.
+  rewrite wp_unfold /wasm_wp_pre=>->. iIntros "H" (σ1 ns κ κs nt) "Hσ".
+  iMod ("H" with "[$]") as %[? Hirr]. iModIntro. iSplit; first done.
+  iIntros (e2 σ2 efs ?). by case: (Hirr κ e2 σ2 efs).
+Qed.
+
+Lemma wp_lift_step s E Φ e1 :
+  to_val e1 = None →
+  (∀ σ1 ns κ κs nt, state_interp σ1 ns (κ ++ κs) nt ={E,∅}=∗
+    ⌜if s is NotStuck then reducible e1 σ1 else True⌝ ∗
+    ▷ ∀ e2 σ2 efs, ⌜prim_step e1 σ1 κ e2 σ2 efs⌝ ={∅,E}=∗
+      ∃ f, state_interp σ2 ns κs (length efs + nt) ∗
+      ↪[frame] f ∗
+      (↪[frame] f -∗ WP e2 @ s; E {{ Φ }}) ∗
+      [∗ list] ef ∈ efs, WP ef @ s; ⊤ {{ fork_post }})
+  ⊢ WP e1 @ s; E {{ Φ }}.
+Proof.
+  iIntros (?) "H". iApply wp_lift_step_fupd; [done|]. iIntros (?????) "Hσ".
+  iMod ("H" with "Hσ") as "[$ H]". iIntros "!> * % !> !>". by iApply "H".
+Qed.
+
+Lemma wp_lift_atomic_step_fupd {s E1 E2 Φ} e1 :
+  iris.to_val e1 = None →
+  (∀ σ1 ns κ κs nt, state_interp σ1 ns (κ ++ κs) nt ={E1}=∗
+    ⌜if s is NotStuck then reducible e1 σ1 else True⌝ ∗
+    ∀ e2 σ2 efs, ⌜prim_step e1 σ1 κ e2 σ2 efs⌝ ={E1}[E2]▷=∗
+      ∃ f, state_interp σ2 ns κs (length efs + nt) ∗
+      ↪[frame] f ∗
+      (↪[frame] f -∗ from_option Φ False (iris.to_val e2)) ∗
+      [∗ list] ef ∈ efs, WP ef @ s; ⊤ {{ fork_post }})
+  ⊢ WP e1 @ s; E1 {{ Φ }}.
+Proof.
+  iIntros (?) "H".
+  iApply (wp_lift_step_fupd s E1 _ e1)=>//; iIntros (σ1 ns κ κs nt) "Hσ1".
+  iMod ("H" $! σ1 with "[$]") as "[$ H]".
+  iApply fupd_mask_intro; first by solve_ndisj.
+  iIntros "Hclose" (e2 σ2 efs ?). iMod "Hclose" as "_".
+  iMod ("H" $! e2 σ2 efs with "[#]") as "H"; [done|].
+  iApply fupd_mask_intro; first solve_ndisj. iIntros "Hclose !>".
+  iMod "Hclose" as "_". iMod "H" as (f1) "($ & Hf1 & HQ & $)".
+  (* This is actually very interesting -- the order of resource consumption
+     is important! *)
+  iModIntro.
+  iExists f1.
+  iFrame.
+  iIntros "?"; iSpecialize ("HQ" with "[$]").
+  destruct (iris.to_val e2) eqn:?; last by iExFalso.
+  iApply wp_value; last done. by apply of_to_val.
+Qed.
+
+Lemma wp_lift_atomic_step {s E Φ} e1 :
+  iris.to_val e1 = None →
+  (∀ σ1 ns κ κs nt, state_interp σ1 ns (κ ++ κs) nt ={E}=∗
+    ⌜if s is NotStuck then reducible e1 σ1 else True⌝ ∗
+    ▷ ∀ e2 σ2 efs, ⌜prim_step e1 σ1 κ e2 σ2 efs⌝ ={E}=∗
+      ∃ f, state_interp σ2 ns κs (length efs + nt) ∗
+      ↪[frame] f ∗         
+      (↪[frame] f -∗ from_option Φ False (iris.to_val e2)) ∗
+      [∗ list] ef ∈ efs, WP ef @ s; ⊤ {{ fork_post }})
+  ⊢ WP e1 @ s; E {{ Φ }}.
+Proof.
+  iIntros (?) "H". iApply wp_lift_atomic_step_fupd; [done|].
+  iIntros (?????) "?". iMod ("H" with "[$]") as "[$ H]".
+  iIntros "!> *". iIntros (Hstep) "!> !>".
+  by iApply "H".
+Qed.
+
+(* A Definition of a context dependent WP for WASM expressions *)
+
+Definition wp_wasm_ctx `{!wfuncG Σ, !wtabG Σ, !wmemG Σ, !wmemsizeG Σ, !wglobG Σ, !wframeG Σ}
+          (s : stuckness) (E : coPset) (e : language.expr wasm_lang)
+           (Φ : val -> iProp Σ) (i : nat) (lh : lholed) : iProp Σ := 
+  ∀ LI, ⌜lfilled i lh e LI⌝ -∗ WP LI @ s; E {{ Φ }}.
+
+
+
+
+Definition wp_wasm_frame `{!wfuncG Σ, !wtabG Σ, !wmemG Σ, !wmemsizeG Σ, !wglobG Σ, !wframeG Σ}
+          (s : stuckness) (E : coPset) (es : language.expr wasm_lang)
+          (Φ : val -> iProp Σ) (n: nat) (f: frame) : iProp Σ :=
+  
+  WP [AI_local n f es] @ s; E {{ Φ }}.
+
+Definition wp_wasm_ctx_frame `{!wfuncG Σ, !wtabG Σ, !wmemG Σ, !wmemsizeG Σ, !wglobG Σ, !wframeG Σ}
+          (s : stuckness) (E : coPset) (es : language.expr wasm_lang)
+          (Φ : val -> iProp Σ) (n: nat) (f: frame) (i : nat) (lh : lholed) : iProp Σ :=
+  
+  ∀ LI, ⌜lfilled i lh es LI⌝ -∗ WP [AI_local n f LI] @ s; E {{ Φ }}.
+
+End Wasm_wp.
+
+
+(* Notations *)
+
+(* Context wps for blocks *)
+Notation "'WP' e @ s ; E 'CTX' i ; lh {{ Φ } }" := (wp_wasm_ctx s E e%E Φ i lh)
+  (at level 20, e, Φ, lh at level 200, only parsing) : bi_scope.
+Notation "'WP' e @ E 'CTX' i ; lh {{ Φ } }" := (wp_wasm_ctx NotStuck E e%E Φ i lh)
+  (at level 20, e, Φ, lh at level 200, only parsing) : bi_scope.
+Notation "'WP' e @ E 'CTX' i ; lh ? {{ Φ } }" := (wp_wasm_ctx MaybeStuck E e%E Φ i lh)
+  (at level 20, e, Φ, lh at level 200, only parsing) : bi_scope.
+Notation "'WP' e 'CTX' i ; lh {{ Φ } }" := (wp_wasm_ctx NotStuck ⊤ e%E Φ i lh)
+  (at level 20, e, Φ, lh at level 200, only parsing) : bi_scope.
+Notation "'WP' e 'CTX' i ; lh ? {{ Φ } }" := (wp_wasm_ctx MaybeStuck ⊤ e%E Φ i lh)
+  (at level 20, e, Φ, lh at level 200, only parsing) : bi_scope.
+Notation "'WP' e @ s ; E 'CTX_EMPTY' {{ Φ } }" := (wp_wasm_ctx s E e%E Φ 0 (LH_base [] []))
+  (at level 20, e, Φ at level 200, only parsing) : bi_scope.
+
+
+Notation "'WP' e @ s ; E 'CTX' i ; lh {{ v , Q } }" := (wp_wasm_ctx s E e%E (λ v, Q) i lh)
+  (at level 20, e, Q, lh at level 200,
+   format "'[hv' 'WP'  e  '/' @  '[' s ;  '/' E  ']' 'CTX'  '/' '[' i ;  '/' lh ']'  '/' {{  '[' v ,  '/' Q  ']' } } ']'") : bi_scope.
+Notation "'WP' e @ s ; E 'CTX_EMPTY' {{ v , Q } }" := (wp_wasm_ctx s E e%E (λ v, Q) 0 (LH_base [] []))
+  (at level 20, e, Q at level 200,
+   format "'[hv' 'WP'  e  '/' @  '[' s ;  '/' E  ']' 'CTX_EMPTY'  '/' {{  '[' v ,  '/' Q  ']' } } ']'") : bi_scope.
+Notation "'WP' e @ E 'CTX' i ; lh {{ v , Q } }" := (wp_wasm_ctx NotStuck E e%E (λ v, Q) i lh)
+  (at level 20, e, Q, lh at level 200,
+   format "'[hv' 'WP'  e  '/' @ '[' E  '/' ']' 'CTX'  '/' '[' i ;  '/' lh ']'  '/' {{  '[' v ,  '/' Q  ']' } } ']'") : bi_scope.
+Notation "'WP' e @ E 'CTX' i ; lh ? {{ v , Q } }" := (wp_wasm_ctx MaybeStuck E e%E (λ v, Q) i lh)
+  (at level 20, e, Q, lh at level 200,
+   format "'[hv' 'WP'  e  '/' @  '[' E  '/' ']' 'CTX'  '/' '[' i ;  '/' lh ']'  '/' ? {{  '[' v ,  '/' Q  ']' } } ']'") : bi_scope.
+Notation "'WP' e 'CTX' i ; lh {{ v , Q } }" := (wp_wasm_ctx NotStuck ⊤ e%E (λ v, Q) i lh)
+  (at level 20, e, Q, lh at level 200,
+   format "'[hv' 'WP'  e  '/' 'CTX'  '/' '[' i ;  '/' lh ']'  '/' {{  '[' v ,  '/' Q  ']' } } ']'") : bi_scope.
+Notation "'WP' e 'CTX' i ; lh ? {{ v , Q } }" := (wp_wasm_ctx MaybeStuck ⊤ e%E (λ v, Q) i lh)
+  (at level 20, e, Q, lh at level 200,
+   format "'[hv' 'WP'  e '/' 'CTX'  '/' '[' i ;  '/' lh ']'  '/' ? {{  '[' v ,  '/' Q  ']' } } ']'") : bi_scope.
+
+(* Frame wps for Local *)
+
+Notation "'WP' e @ s ; E 'FRAME' n ; f {{ Φ } }" := (wp_wasm_frame s E e%E Φ n f)
+  (at level 20, only parsing) : bi_scope.
+
+Notation "'WP' e @ s ; E 'FRAME' n ; f {{ v , Q } }" := (wp_wasm_frame s E e%E (λ v, Q) n f)
+  (at level 20, e, Q, n, f at level 200,
+    format "'[hv' 'WP'  e  '/' @  '[' s ;  '/' E  ']' 'FRAME'  '/' '[' n ;  '/' f ']'  '/' {{  '[' v ,  '/' Q  ']' } } ']'") : bi_scope.
+
+Notation "'WP' e @ s ; E 'FRAME' n ; f 'CTX' i ; lh {{ v , Q } }" := (wp_wasm_ctx_frame s E e%E (λ v, Q) n f i lh)
+  (at level 20, e, Q, lh at level 200,
+   format "'[hv' 'WP'  e  '/' @  '[' s ;  '/' E  ']' 'FRAME'  '/' '[' n ;  '/' f ']'  '/' 'CTX'  '/' '[' i ;  '/' lh ']'  '/' {{  '[' v ,  '/' Q  ']' } } ']'") : bi_scope.
+Notation "'WP' e @ s ; E 'FRAME' n ; f 'CTX_EMPTY' {{ v , Q } }" := (wp_wasm_ctx_frame s E e%E (λ v, Q) n f 0 (LH_base [] []))
+  (at level 20, e, Q at level 200,
+   format "'[hv' 'WP'  e  '/' @  '[' s ;  '/' E  ']' 'FRAME'  '/' '[' n ;  '/' f ']'  '/' 'CTX_EMPTY'  '/' {{  '[' v ,  '/' Q  ']' } } ']'") : bi_scope.
+Notation "'WP' e @ E 'FRAME' n ; f 'CTX' i ; lh {{ v , Q } }" := (wp_wasm_ctx_frame NotStuck E e%E (λ v, Q) n f i lh)
+  (at level 20, e, Q, lh at level 200,
+   format "'[hv' 'WP'  e  '/' @ '[' E  '/' ']' 'FRAME'  '/' '[' n ;  '/' f ']'  '/' 'CTX'  '/' '[' i ;  '/' lh ']'  '/' {{  '[' v ,  '/' Q  ']' } } ']'") : bi_scope.
+Notation "'WP' e @ E 'FRAME' n ; f 'CTX' i ; lh ? {{ v , Q } }" := (wp_wasm_ctx_frame MaybeStuck E e%E (λ v, Q) n f i lh)
+  (at level 20, e, Q, lh at level 200,
+   format "'[hv' 'WP'  e  '/' @  '[' E  '/' ']' 'FRAME'  '/' '[' n ;  '/' f ']'  '/' 'CTX'  '/' '[' i ;  '/' lh ']'  '/' ? {{  '[' v ,  '/' Q  ']' } } ']'") : bi_scope.
+Notation "'WP' e 'FRAME' n ; f 'CTX' i ; lh {{ v , Q } }" := (wp_wasm_ctx_frame NotStuck ⊤ e%E (λ v, Q) n f i lh)
+  (at level 20, e, Q, lh at level 200,
+   format "'[hv' 'WP'  e  '/' 'FRAME'  '/' '[' n ;  '/' f ']'  '/' 'CTX'  '/' '[' i ;  '/' lh ']'  '/' {{  '[' v ,  '/' Q  ']' } } ']'") : bi_scope.
+Notation "'WP' e 'FRAME' n ; f 'CTX' i ; lh ? {{ v , Q } }" := (wp_wasm_ctx_frame MaybeStuck ⊤ e%E (λ v, Q) n f i lh)
+  (at level 20, e, Q, lh at level 200,
+   format "'[hv' 'WP'  e '/' 'FRAME'  '/' '[' n ;  '/' f ']'  '/' 'CTX'  '/' '[' i ;  '/' lh ']'  '/' ? {{  '[' v ,  '/' Q  ']' } } ']'") : bi_scope.
