theories/iris_wp_pure.v
@@ -1,0 +1,331 @@
+From mathcomp Require Import ssreflect eqtype seq ssrbool.
+From iris.program_logic Require Import language.
+From iris.proofmode Require Import base tactics classes.
+From iris.base_logic Require Export gen_heap ghost_map proph_map.
+From iris.base_logic.lib Require Export fancy_updates.
+From iris.bi Require Export weakestpre.
+Require Export iris iris_locations iris_properties iris_atomicity iris_wp_def stdpp_aux.
+Require Export datatypes host operations properties opsem.
+
+
+(* basic instructions with simple(pure) reductions *)
+
+(* numerics *)
+Lemma wp_unop (s : stuckness) (E : coPset) (Φ : val -> iProp Σ) (v v' : value) (t: value_type) (op: unop) f0:
+  app_unop op v = v' ->
+  ↪[frame] f0 -∗
+   Φ (immV [v']) -∗
+  WP [AI_basic (BI_const v); AI_basic (BI_unop t op)] @ s; E {{ v, Φ v ∗ ↪[frame] f0 }}.
+Proof.
+  iIntros (Hunop) "Hf HΦ".
+  iApply wp_lift_atomic_step. simpl ; trivial.
+  iIntros (σ ns κ κs nt) "Hσ !>".
+  iSplit.
+  - iPureIntro.
+    destruct s => //=.
+    unfold language.reducible, language.prim_step => /=.
+    exists [], [AI_basic (BI_const v')], σ, [].
+    destruct σ as [[[ hs ws] locs] inst].
+    unfold iris.prim_step => /=.
+    repeat split => //. apply r_simple. rewrite <- Hunop. apply rs_unop.
+  - destruct σ as [[[hs ws] locs] inst].
+    iIntros "!>" (es σ2 efs HStep) "!>".
+    destruct σ2 as [[[hs' ws'] locs'] inst'].
+    destruct HStep as (H & -> & ->).
+    only_one_reduction H.
+Qed.
+ 
+Lemma wp_binop (s : stuckness) (E : coPset) (Φ : val -> iProp Σ) (v1 v2 v : value) (t: value_type) (op: binop) f0:
+  app_binop op v1 v2 = Some v ->
+  ↪[frame] f0 -∗
+  Φ (immV [v]) -∗
+  WP [AI_basic (BI_const v1); AI_basic (BI_const v2); AI_basic (BI_binop t op)] @ s; E {{ v, Φ v ∗ ↪[frame] f0 }}.
+Proof.
+  iIntros (Hbinop) "Hf HΦ".
+  iApply wp_lift_atomic_step => //=.
+  iIntros (σ ns κ κs nt) "Hσ !>".
+  iSplit.
+  - iPureIntro.
+    destruct s => //=.
+    unfold reducible, language.prim_step => /=.
+    exists [], [AI_basic (BI_const v)], σ, [].
+    destruct σ as [[[hs ws] locs] inst].
+    unfold iris.prim_step => /=.
+    repeat split => //.
+    apply r_simple.
+    by apply rs_binop_success.
+  - destruct σ as [[[hs ws] locs] inst] => //=.
+    iIntros "!>" (es σ2 efs HStep) "!>".
+    destruct σ2 as [[[hs' ws'] locs'] inst'] => //=.
+    destruct HStep as [H [-> ->]].
+    only_one_reduction H.
+Qed.
+                                                                  
+
+Lemma wp_binop_failure (s : stuckness) (E : coPset) (Φ : val -> iProp Σ) (v1 v2 : value) (t: value_type) (op: binop) f0:
+  app_binop op v1 v2 = None ->
+  Φ trapV -∗
+  ↪[frame] f0 -∗
+  WP [AI_basic (BI_const v1); AI_basic (BI_const v2); AI_basic (BI_binop t op)] @ s; E {{ v, Φ v ∗ ↪[frame] f0 }}.
+Proof.
+  iIntros (Hbinop) "Hf HΦ".
+  iApply wp_lift_atomic_step => //=.
+  iIntros (σ ns κ κs nt) "Hσ".
+  iModIntro.
+  iSplit.
+  - iPureIntro.
+    destruct s => //=.
+    unfold reducible, language.prim_step => /=.
+    exists [], [AI_trap], σ, [].
+    destruct σ as [[[hs ws] locs] inst].
+    unfold iris.prim_step => /=.
+    repeat split => //.
+    apply r_simple.
+    by apply rs_binop_failure.
+  - destruct σ as [[[hs ws] locs] inst] => //=.
+    iIntros "!>" (es σ2 efs HStep) "!>".
+    destruct σ2 as [[[hs' ws'] locs'] inst'] => //=.
+    destruct HStep as [H [-> ->]].
+    only_one_reduction H.
+Qed.
+    
+Lemma wp_relop (s : stuckness) (E : coPset) (Φ : val -> iProp Σ) (v1 v2 : value) (b: bool) (t: value_type) (op: relop) f0:
+  app_relop op v1 v2 = b ->
+  ↪[frame] f0 -∗
+  Φ (immV [(VAL_int32 (wasm_bool b))]) -∗
+  WP [AI_basic (BI_const v1); AI_basic (BI_const v2); AI_basic (BI_relop t op)] @ s; E {{ v, Φ v }}.
+Proof.
+  iIntros (Hrelop) "Hf HΦ".
+  iApply wp_lift_atomic_step => //=.
+  iIntros (σ ns κ κs nt) "Hσ !>".
+  iSplit.
+  - iPureIntro.
+    destruct s => //=.
+    unfold reducible, language.prim_step => /=.
+    exists [], [AI_basic (BI_const (VAL_int32 (wasm_bool b)))], σ, [].
+    destruct σ as [[[hs ws] locs] inst].
+    unfold iris.prim_step => /=.
+    repeat split => //.
+    apply r_simple.
+    subst.
+    by apply rs_relop.
+  - destruct σ as [[[hs ws] locs] inst] => //=.
+    iIntros "!>" (es σ2 efs HStep) "!>".
+    destruct σ2 as [[[hs' ws'] locs'] inst'] => //=.
+    destruct HStep as [H [-> ->]].
+    only_one_reduction H.
+Qed.
+
+Lemma wp_testop_i32 (s : stuckness) (E : coPset) (Φ : val -> iProp Σ) (v : i32) (b: bool) (t: value_type) (op: testop) f0:
+  app_testop_i (e:=i32t) op v = b ->
+  ↪[frame] f0 -∗
+  Φ (immV [(VAL_int32 (wasm_bool b))]) -∗
+    WP [AI_basic (BI_const (VAL_int32 v)); AI_basic (BI_testop T_i32 op)] @ s; E {{ v, Φ v ∗ ↪[frame] f0 }}.
+Proof.
+  iIntros (Htestop) "Hf0 HΦ".
+  iApply wp_lift_atomic_step => //=.
+  iIntros (σ ns κ κs nt) "Hσ !>".
+  iSplit.
+  - iPureIntro.
+    destruct s => //=.
+    unfold reducible, language.prim_step => /=.
+    exists [], [AI_basic (BI_const (VAL_int32 (wasm_bool b)))], σ, [].
+    destruct σ as [[[hs ws] locs] inst].
+    unfold iris.prim_step => /=.
+    repeat split => //.
+    apply r_simple.
+    subst.
+    by apply rs_testop_i32.
+  - destruct σ as [[[hs ws] locs] inst] => //=.
+    iIntros "!>" (es σ2 efs HStep) "!>".
+    destruct σ2 as [[[hs' ws'] locs'] inst'] => //=.
+    destruct HStep as [H [-> ->]].
+    only_one_reduction H.
+Qed.
+
+Lemma wp_testop_i64 (s : stuckness) (E : coPset) (Φ : val -> iProp Σ) (v : i64) (b: bool) (t: value_type) (op: testop) f0:
+  app_testop_i (e:=i64t) op v = b ->
+  ↪[frame] f0 -∗
+  Φ (immV [(VAL_int32 (wasm_bool b))]) -∗
+    WP [AI_basic (BI_const (VAL_int64 v)); AI_basic (BI_testop T_i64 op)] @ s; E {{ v, Φ v ∗ ↪[frame] f0}}.
+Proof.
+  iIntros (Htestop) "Hf0 HΦ".
+  iApply wp_lift_atomic_step => //=.
+  iIntros (σ ns κ κs nt) "Hσ !>".
+  iSplit.
+  - iPureIntro.
+    destruct s => //=.
+    unfold reducible, language.prim_step => /=.
+    exists [], [AI_basic (BI_const (VAL_int32 (wasm_bool b)))], σ, [].
+    destruct σ as [[[hs ws] locs] inst].
+    unfold iris.prim_step => /=.
+    repeat split => //.
+    apply r_simple.
+    subst.
+    by apply rs_testop_i64.
+  - destruct σ as [[[hs ws] locs] inst] => //=.
+    iIntros "!>" (es σ2 efs HStep) "!>".
+    destruct σ2 as [[[hs' ws'] locs'] inst'] => //=.
+    destruct HStep as [H [-> ->]].
+    only_one_reduction H.
+Qed.
+
+Lemma wp_cvtop_convert (s : stuckness) (E : coPset) (Φ : val -> iProp Σ) (v v': value) (t1 t2: value_type) (sx: option sx) f0:
+  cvt t2 sx v = Some v' ->
+  types_agree t1 v ->
+  ↪[frame] f0 -∗
+  Φ (immV [v']) -∗
+    WP [AI_basic (BI_const v); AI_basic (BI_cvtop t2 CVO_convert t1 sx)] @ s; E {{ v, Φ v ∗ ↪[frame] f0}}.
+Proof.
+  iIntros (Hcvtop Htype) "Hf0 HΦ".
+  iApply wp_lift_atomic_step => //=.
+  iIntros (σ ns κ κs nt) "Hσ !>".
+  iSplit.
+  - iPureIntro.
+    destruct s => //=.
+    unfold reducible, language.prim_step => /=.
+    exists [], [AI_basic (BI_const v')], σ, [].
+    destruct σ as [[[hs ws] locs] inst].
+    unfold iris.prim_step => /=.
+    repeat split => //.
+    apply r_simple.
+    subst.
+    by apply rs_convert_success.
+  - destruct σ as [[[hs ws] locs] inst] => //=.
+    iIntros "!>" (es σ2 efs HStep) "!>".
+    destruct σ2 as [[[hs' ws'] locs'] inst'] => //=.
+    destruct HStep as [H [-> ->]].
+    only_one_reduction H.
+Qed.
+
+Lemma wp_cvtop_reinterpret (s : stuckness) (E : coPset) (Φ : val -> iProp Σ) (v v': value) (t1 t2: value_type) f0:
+  wasm_deserialise (bits v) t2 = v' ->
+  types_agree t1 v ->
+  ↪[frame] f0 -∗
+  Φ (immV [v']) -∗
+    WP [AI_basic (BI_const v); AI_basic (BI_cvtop t2 CVO_reinterpret t1 None)] @ s; E {{ v, Φ v ∗ ↪[frame] f0}}.
+Proof.
+  iIntros (Hcvtop Htype) "Hf0 HΦ".
+  iApply wp_lift_atomic_step => //=.
+  iIntros (σ ns κ κs nt) "Hσ !>".
+  iSplit.
+  - iPureIntro.
+    destruct s => //=.
+    unfold reducible, language.prim_step => /=.
+    exists [], [AI_basic (BI_const v')], σ, [].
+    destruct σ as [[[hs ws] locs] inst].
+    unfold iris.prim_step => /=.
+    repeat split => //.
+    apply r_simple.
+    subst.
+    by apply rs_reinterpret.
+  - destruct σ as [[[hs ws] locs] inst] => //=.
+    iIntros "!>" (es σ2 efs HStep) "!>".
+    destruct σ2 as [[[hs' ws'] locs'] inst'] => //=.
+    destruct HStep as [H [-> ->]].
+    only_one_reduction H.
+Qed.
+
+(* Non-numerics -- stack operations, control flows *)
+
+Lemma wp_nop (s : stuckness) (E : coPset) (Φ : val -> iProp Σ) f0:
+  ↪[frame] f0 -∗
+  Φ (immV []) -∗
+    WP [AI_basic (BI_nop)] @ s; E {{ v, Φ v ∗ ↪[frame] f0}}.
+Proof.
+  iIntros "Hf0 HΦ".
+  iApply wp_lift_atomic_step => //=.
+  iIntros (σ ns κ κs nt) "Hσ !>".
+  iSplit.
+  - iPureIntro.
+    destruct s => //=.
+    unfold reducible, language.prim_step => /=.
+    exists [], [], σ, [].
+    destruct σ as [[[hs ws] locs] inst].
+    unfold iris.prim_step => /=.
+    repeat split => //.
+    apply r_simple.
+    subst.
+    by apply rs_nop.
+  - destruct σ as [[[hs ws] locs] inst] => //=.
+    iIntros "!>" (es σ2 efs HStep) "!>".
+    destruct σ2 as [[[hs' ws'] locs'] inst'] => //=.
+    destruct HStep as [H [-> ->]].
+    only_one_reduction H.
+Qed.
+
+
+
+
+Lemma wp_drop (s : stuckness) (E : coPset) (Φ : val -> iProp Σ) v f0 :
+  ↪[frame] f0 -∗
+  Φ (immV []) -∗
+    WP [AI_basic (BI_const v) ; AI_basic BI_drop] @ s; E {{ w, Φ w ∗ ↪[frame] f0}}.
+Proof.
+  iIntros "Hf0 HΦ".
+  iApply wp_lift_atomic_step. simpl ; trivial.
+  iIntros (σ ns κ κs nt) "Hσ !>".
+  iSplit.
+  - iPureIntro.
+    destruct s => //=.
+    unfold language.reducible, language.prim_step => /=.
+    exists [], [], σ, [].
+    destruct σ as [[[ hs ws ] locs ] inst ].
+    unfold iris.prim_step => /=.
+    repeat split => //.
+    apply r_simple ; apply rs_drop.
+  - destruct σ as [[[ hs ws ] locs ] inst ].
+    iIntros "!>" (es σ2 efs HStep) "!>".
+    destruct σ2 as [[[ hs' ws' ] locs' ] inst'].
+    destruct HStep as (H & -> & ->).
+    only_one_reduction H.
+Qed.
+
+Lemma wp_select_false (s: stuckness) (E :coPset) (Φ : val -> iProp Σ) n v1 v2 f0 :
+  n = Wasm_int.int_zero i32m ->
+  ↪[frame] f0 -∗
+  Φ (immV [v2]) -∗ WP [AI_basic (BI_const v1) ; AI_basic (BI_const v2) ;
+                      AI_basic (BI_const (VAL_int32 n)) ; AI_basic (BI_select) ] @ s;
+E {{ w, Φ w ∗ ↪[frame] f0}}.
+Proof.
+  iIntros (Hn) "Hf0 HΦ".
+  iApply wp_lift_atomic_step. simpl ; trivial.
+  iIntros (σ ns κ κs nt) "Hσ !>".
+  iSplit.
+  - iPureIntro.
+    destruct s => //=.
+    unfold language.reducible, language.prim_step => /=.
+    exists [], [AI_basic (BI_const v2)], σ, [].
+    destruct σ as [[[ hs ws ] locs ] inst].
+    unfold iris.prim_step => /=. repeat split => //.
+    apply r_simple ; by apply rs_select_false.
+  - destruct σ as [[[ hs ws ] locs ] inst ].
+    iIntros "!>" (es σ2 efs HStep) "!>".
+    destruct σ2 as [[[ hs' ws' ] locs' ] inst'].
+    destruct HStep as (H & -> & ->).
+    only_one_reduction H.
+Qed.
+
+Lemma wp_select_true (s: stuckness) (E : coPset) (Φ: val -> iProp Σ) n v1 v2 f0 :
+  n <> Wasm_int.int_zero i32m ->
+  ↪[frame] f0 -∗
+  Φ (immV [v1]) -∗ WP [AI_basic (BI_const v1) ; AI_basic (BI_const v2) ;
+                      AI_basic (BI_const (VAL_int32 n)) ; AI_basic (BI_select) ] @ s;
+E {{ w, Φ w ∗ ↪[frame] f0}}.
+Proof.
+  iIntros (Hn) "Hf0 HΦ".
+  iApply wp_lift_atomic_step => //=.
+  iIntros (σ ns κ κs nt) "Hσ !>".
+  iSplit.
+  - iPureIntro. destruct s => //=. unfold language.reducible, language.prim_step => /=.
+    exists [], [AI_basic (BI_const v1)], σ, [].
+    destruct σ as [[[ hs ws ] locs ] inst].
+    unfold iris.prim_step => /=. repeat split => //.
+    apply r_simple ; by apply rs_select_true.
+  - destruct σ as [[[ hs ws ] locs ] inst].
+    iIntros "!>" (es σ2 efs HStep) "!>".
+    destruct σ2 as [[[ hs' ws' ] locs' ] inst'].
+    destruct HStep as (H & -> & ->).
+    only_one_reduction H.
+Qed.
+    
